{
  "metadata": {
    "title": "EPD Calculation Engine Input Payload",
    "generated_at": "2026-09-22T10:17:43.334014",
    "methodology": "ef31",
    "database_version": "ecoinvent v3.12 Cut-off",
    "standard": "EN 15804+A2:2019 / ISO 14025:2006"
  },
  "project_info": {
    "product_name": "Carrier AquaEdge 19DV Centrifugal Chiller",
    "manufacturer_name": "Declared Manufacturer",
    "functional_unit": "1 unit over 25 years reference service life (500.0 RT)",
    "declared_unit": "1 piece",
    "pcr_ref": "UL 10010-4 Part B & EN 15804+A2",
    "geography": "Global",
    "lifespan_years": 25
  },
  "stages_data": {
    "A1_BOM": [
      {
        "id": "pdf-1-1",
        "name": "Compressor Volute & Casting",
        "material": "steel_hot_rolled",
        "mass": 2250,
        "unit": "kg",
        "ecoinvent_id": "ecoinvent_row_15528",
        "supplier": "Midwest Iron Works",
        "transport_km": 420,
        "module": "A1",
        "dataset": "market for steel, low-alloyed, hot rolled [GLO]",
        "reference_product_name": "steel, low-alloyed, hot rolled",
        "ecoinvent_row": 15528,
        "ecoinvent_geography": "GLO",
        "ecoinvent_matched": true,
        "provider_id": "ecoinvent_row_15528",
        "reference_unit": "kg"
      },
      {
        "id": "pdf-1-2",
        "name": "Evaporator & Condenser Tubes",
        "material": "copper_tube_wire",
        "mass": 720,
        "unit": "kg",
        "ecoinvent_id": "ecoinvent_row_10657",
        "supplier": "Great Lakes Copper Corp",
        "transport_km": 280,
        "module": "A1",
        "dataset": "market for copper slag [GLO]",
        "reference_product_name": "copper slag",
        "ecoinvent_row": 10657,
        "ecoinvent_geography": "GLO",
        "ecoinvent_matched": true,
        "provider_id": "ecoinvent_row_10657",
        "reference_unit": "kg"
      },
      {
        "id": "pdf-1-3",
        "name": "Semi-Hermetic Induction Motor",
        "material": "electric_motor_industrial",
        "mass": 480,
        "unit": "kg",
        "ecoinvent_id": "ecoinvent_row_10882",
        "supplier": "ElectroMotors Industrial",
        "transport_km": 650,
        "module": "A1",
        "dataset": "market for electric kettle [GLO]",
        "reference_product_name": "electric kettle",
        "ecoinvent_row": 10882,
        "ecoinvent_geography": "GLO",
        "ecoinvent_matched": true,
        "provider_id": "ecoinvent_row_10882",
        "reference_unit": "kg"
      },
      {
        "id": "pdf-1-4",
        "name": "Shell Thermal PUF Insulation",
        "material": "insulation_polyurethane_rigid",
        "mass": 140,
        "unit": "kg",
        "ecoinvent_id": "ecoinvent_row_14055",
        "supplier": "FoamTech Insulation",
        "transport_km": 190,
        "module": "A1",
        "dataset": "market for polyurethane adhesive [GLO]",
        "reference_product_name": "polyurethane adhesive",
        "ecoinvent_row": 14055,
        "ecoinvent_geography": "GLO",
        "ecoinvent_matched": true,
        "provider_id": "ecoinvent_row_14055",
        "reference_unit": "kg"
      },
      {
        "id": "pdf-1-5",
        "name": "Power Inverter & Solid-State VFD",
        "material": "electronics_vfd",
        "mass": 110,
        "unit": "kg",
        "ecoinvent_id": "ecoinvent_row_11483",
        "supplier": "Advantech Power Systems",
        "transport_km": 890,
        "module": "A1",
        "dataset": "market for electronics scrap [GLO]",
        "reference_product_name": "electronics scrap",
        "ecoinvent_row": 11483,
        "ecoinvent_geography": "GLO",
        "ecoinvent_matched": true,
        "provider_id": "ecoinvent_row_11483",
        "reference_unit": "kg"
      },
      {
        "id": "pdf-1-6",
        "name": "Microchannel Subcooler Coil",
        "material": "aluminium_cast_alloy",
        "mass": 95,
        "unit": "kg",
        "ecoinvent_id": "ecoinvent_row_9452",
        "supplier": "Alloy Heat Exchangers",
        "transport_km": 350,
        "module": "A1",
        "dataset": "market for aluminium, cast alloy [GLO]",
        "reference_product_name": "aluminium, cast alloy",
        "ecoinvent_row": 9452,
        "ecoinvent_geography": "GLO",
        "ecoinvent_matched": true,
        "provider_id": "ecoinvent_row_9452",
        "reference_unit": "kg"
      },
      {
        "id": "pdf-1-7",
        "name": "Refrigerant High-Pressure Piping",
        "material": "steel_stainless_304",
        "mass": 85,
        "unit": "kg",
        "ecoinvent_id": "ecoinvent_row_11757",
        "supplier": "Precision Alloy Tubing",
        "transport_km": 340,
        "module": "A1",
        "dataset": "market for forging, steel [GLO]",
        "reference_product_name": "forging, steel",
        "ecoinvent_row": 11757,
        "ecoinvent_geography": "GLO",
        "ecoinvent_matched": true,
        "provider_id": "ecoinvent_row_11757",
        "reference_unit": "kg"
      },
      {
        "id": "pdf-1-8",
        "name": "Base Skid Frame & Mounts",
        "material": "steel_hot_rolled",
        "mass": 540,
        "unit": "kg",
        "ecoinvent_id": "ecoinvent_row_15528",
        "supplier": "ArcelorMittal Midwest",
        "transport_km": 260,
        "module": "A1",
        "dataset": "market for steel, low-alloyed, hot rolled [GLO]",
        "reference_product_name": "steel, low-alloyed, hot rolled",
        "ecoinvent_row": 15528,
        "ecoinvent_geography": "GLO",
        "ecoinvent_matched": true,
        "provider_id": "ecoinvent_row_15528",
        "reference_unit": "kg"
      }
    ],
    "A2_Transport": [
      {
        "id": "a2-leg-1",
        "name": "Zurich Foundry Ltd (Genoa Port, Italy)",
        "mode": "Freight Train (Electric/Diesel)",
        "distance": 450,
        "dist": 450,
        "mass_kg": 2250.0,
        "emission_factor": 0.035,
        "ef": 0.035,
        "module": "A2",
        "provider_id": "ecoinvent_transport_freight_train_rer",
        "reference_unit": "tkm",
        "linked_material_ids": []
      },
      {
        "id": "a2-leg-2",
        "name": "Mediterranean Shipping Co (Port of New York, USA)",
        "mode": "Transoceanic Container Ship",
        "distance": 6200,
        "dist": 6200,
        "mass_kg": 2250.0,
        "emission_factor": 0.0145,
        "ef": 0.0145,
        "module": "A2",
        "provider_id": "ecoinvent_transport_container_ship_glo",
        "reference_unit": "tkm",
        "linked_material_ids": []
      },
      {
        "id": "a2-leg-3",
        "name": "Great Lakes Intermodal (Assembly Plant, Chicago IL)",
        "mode": "Freight Train (Electric/Diesel)",
        "distance": 900,
        "dist": 900,
        "mass_kg": 2250.0,
        "emission_factor": 0.035,
        "ef": 0.035,
        "module": "A2",
        "provider_id": "ecoinvent_transport_freight_train_rer",
        "reference_unit": "tkm",
        "linked_material_ids": []
      },
      {
        "id": "a2-leg-4",
        "name": "Wieland Copper Mill (Rotterdam Port, Netherlands)",
        "mode": "Heavy Lorry >32t (EURO 6)",
        "distance": 620,
        "dist": 620,
        "mass_kg": 720.0,
        "emission_factor": 0.088,
        "ef": 0.088,
        "module": "A2",
        "provider_id": "ecoinvent_transport_lorry_32t_rer",
        "reference_unit": "tkm",
        "linked_material_ids": []
      },
      {
        "id": "a2-leg-5",
        "name": "Atlantic Carrier Line (Montreal Port, Canada)",
        "mode": "Transoceanic Container Ship",
        "distance": 5850,
        "dist": 5850,
        "mass_kg": 720.0,
        "emission_factor": 0.0145,
        "ef": 0.0145,
        "module": "A2",
        "provider_id": "ecoinvent_transport_container_ship_glo",
        "reference_unit": "tkm",
        "linked_material_ids": []
      },
      {
        "id": "a2-leg-6",
        "name": "Advantech Electronics (Long Beach Port, USA)",
        "mode": "Transoceanic Container Ship",
        "distance": 10800,
        "dist": 10800,
        "mass_kg": 110.0,
        "emission_factor": 0.0145,
        "ef": 0.0145,
        "module": "A2",
        "provider_id": "ecoinvent_transport_container_ship_glo",
        "reference_unit": "tkm",
        "linked_material_ids": []
      },
      {
        "id": "a2-leg-7",
        "name": "US Pacific Trucking (Assembly Plant, Chicago IL)",
        "mode": "Heavy Lorry >32t (EURO 6)",
        "distance": 3250,
        "dist": 3250,
        "mass_kg": 110.0,
        "emission_factor": 0.088,
        "ef": 0.088,
        "module": "A2",
        "provider_id": "ecoinvent_transport_lorry_32t_rer",
        "reference_unit": "tkm",
        "linked_material_ids": []
      },
      {
        "id": "a2-leg-8",
        "name": "ArcelorMittal Midwest (Assembly Plant, Chicago IL)",
        "mode": "Heavy Lorry >32t (EURO 6)",
        "distance": 85,
        "dist": 85,
        "mass_kg": 540.0,
        "emission_factor": 0.088,
        "ef": 0.088,
        "module": "A2",
        "provider_id": "ecoinvent_transport_lorry_32t_rer",
        "reference_unit": "tkm",
        "linked_material_ids": []
      },
      {
        "id": "a2-leg-9",
        "name": "Armacell Polymer Systems (Assembly Plant, Chicago IL)",
        "mode": "Heavy Lorry >32t (EURO 6)",
        "distance": 1120,
        "dist": 1120,
        "mass_kg": 140.0,
        "emission_factor": 0.088,
        "ef": 0.088,
        "module": "A2",
        "provider_id": "ecoinvent_transport_lorry_32t_rer",
        "reference_unit": "tkm",
        "linked_material_ids": []
      }
    ],
    "A3_Manufacturing": {
      "annual_facility_kwh": 34000,
      "natural_gas_mj": 0,
      "grid_region": "US_Average",
      "water_m3": 0,
      "electricity_provider_id": "ecoinvent_elec_mv_us",
      "gas_provider_id": "ecoinvent_gas_burned_boiler_glo",
      "water_provider_id": "ecoinvent_water_deionised_glo",
      "annual_production_units": 1000.0,
      "electricity_provider_id_reference_unit": "kWh",
      "gas_provider_id_reference_unit": "MJ",
      "water_provider_id_reference_unit": "m3"
    },
    "A4_A5_Installation": {
      "outbound_transport_km": 750,
      "transport_mode": "Heavy Lorry >32t (EURO 6)",
      "installation_energy_kwh": 350,
      "commissioning_refrigerant_loss_kg": 0.5,
      "rigging_crane_diesel_liters": 37.8,
      "outbound_provider_id": "ecoinvent_transport_lorry_32t_rer",
      "installation_energy_provider_id": "ecoinvent_elec_mv_us",
      "consumable_provider_id": "ecoinvent_diesel_burned_building_machine_glo",
      "outbound_provider_id_reference_unit": "tkm",
      "installation_energy_provider_id_reference_unit": "kWh",
      "consumable_provider_id_reference_unit": "MJ"
    },
    "B1_B7_Operational": {
      "refrigerant_type": "R134A",
      "refrigerant_charge_kg": 45,
      "annual_leak_rate_percent": 2,
      "fugitive_operational_leak_rate": 0,
      "efficiency_kw_per_ton": 0.54,
      "capacity_rt": 500.0,
      "target_cities": [],
      "cooling_tower_water_m3_yr": 120,
      "scheduled_maintenance_kwh_yr": 0,
      "major_component_replacement_year": 15,
      "iplv_kw_per_ton": 0.435,
      "refrigerant_gwp_cf": 1430.0,
      "energy_provider_id": "ecoinvent_elec_mv_us",
      "water_provider_id": "ecoinvent_water_deionised_glo",
      "energy_provider_id_reference_unit": "kWh",
      "water_provider_id_reference_unit": "m3",
      "annual_operating_hours": 8760.0,
      "load_basis": "full_load",
      "rsl_years": 25.0,
      "city_grid_providers": {
        "Chicago": "ecoinvent_elec_mv_us",
        "Houston": "ecoinvent_elec_tx",
        "Frankfurt": "ecoinvent_elec_de",
        "Dubai": "ecoinvent_elec_ae"
      },
      "city_grid_providers_reference_units": {
        "Chicago": "kWh",
        "Houston": "kWh",
        "Frankfurt": "kWh",
        "Dubai": "kWh"
      }
    },
    "B2_Maintenance": {
      "consumable_mass_kg": 25,
      "provider_id": "ecoinvent_lubricating_oil_glo",
      "maintenance_cycles_per_rsl": 25.0,
      "reference_unit": "kg"
    },
    "B3_Repair": {
      "repair_events_per_rsl": 0,
      "replaced_part_name": "",
      "part_mass_kg": 0,
      "material_type": "",
      "provider_id": "ecoinvent_steel_hot_rolled_glo",
      "reference_unit": "kg"
    },
    "B4_Replacement": {
      "esl_years": 25
    },
    "B5_Refurbishment": {
      "refurbishment_events_per_rsl": 0,
      "material_name": "",
      "mass_kg": 0,
      "provider_id": "ecoinvent_copper_tube_wire_glo",
      "reference_unit": "kg"
    },
    "C1_C4_EndOfLife": {
      "recycling_rate_percent": 92.4,
      "landfill_rate_percent": 4.5,
      "incineration_rate_percent": 3.1,
      "decommissioning_energy_kwh": 120,
      "waste_transport_km": 100,
      "deconstruction_provider_id": "ecoinvent_diesel_dismantling_glo",
      "waste_transport_provider_id": "ecoinvent_transport_lorry_32t_rer",
      "recycling_process_provider_id": "ecoinvent_waste_metal_recycling_glo",
      "incineration_process_provider_id": "ecoinvent_waste_incineration_glo",
      "landfill_process_provider_id": "ecoinvent_waste_landfill_glo",
      "deconstruction_provider_id_reference_unit": "MJ",
      "waste_transport_provider_id_reference_unit": "tkm",
      "recycling_process_provider_id_reference_unit": "kg",
      "incineration_process_provider_id_reference_unit": "kg",
      "landfill_process_provider_id_reference_unit": "kg"
    },
    "D_Circularity": {
      "virgin_material_provider_id": "ecoinvent_virgin_steel_primary_glo",
      "recycled_process_provider_id": "ecoinvent_secondary_steel_electric_glo",
      "overall_recovery_rate_percent": 90.0,
      "virgin_material_provider_id_reference_unit": "kg",
      "recycled_process_provider_id_reference_unit": "kWh"
    }
  },
  "full_payload": {
    "extracted_data": {
      "bom": [
        {
          "id": "pdf-1-1",
          "name": "Compressor Volute & Casting",
          "material": "steel_hot_rolled",
          "mass": 2250,
          "unit": "kg",
          "ecoinvent_id": "ecoinvent_row_15528",
          "supplier": "Midwest Iron Works",
          "transport_km": 420,
          "module": "A1",
          "dataset": "market for steel, low-alloyed, hot rolled [GLO]",
          "reference_product_name": "steel, low-alloyed, hot rolled",
          "ecoinvent_row": 15528,
          "ecoinvent_geography": "GLO",
          "ecoinvent_matched": true
        },
        {
          "id": "pdf-1-2",
          "name": "Evaporator & Condenser Tubes",
          "material": "copper_tube_wire",
          "mass": 720,
          "unit": "kg",
          "ecoinvent_id": "ecoinvent_row_10657",
          "supplier": "Great Lakes Copper Corp",
          "transport_km": 280,
          "module": "A1",
          "dataset": "market for copper slag [GLO]",
          "reference_product_name": "copper slag",
          "ecoinvent_row": 10657,
          "ecoinvent_geography": "GLO",
          "ecoinvent_matched": true
        },
        {
          "id": "pdf-1-3",
          "name": "Semi-Hermetic Induction Motor",
          "material": "electric_motor_industrial",
          "mass": 480,
          "unit": "kg",
          "ecoinvent_id": "ecoinvent_row_10882",
          "supplier": "ElectroMotors Industrial",
          "transport_km": 650,
          "module": "A1",
          "dataset": "market for electric kettle [GLO]",
          "reference_product_name": "electric kettle",
          "ecoinvent_row": 10882,
          "ecoinvent_geography": "GLO",
          "ecoinvent_matched": true
        },
        {
          "id": "pdf-1-4",
          "name": "Shell Thermal PUF Insulation",
          "material": "insulation_polyurethane_rigid",
          "mass": 140,
          "unit": "kg",
          "ecoinvent_id": "ecoinvent_row_14055",
          "supplier": "FoamTech Insulation",
          "transport_km": 190,
          "module": "A1",
          "dataset": "market for polyurethane adhesive [GLO]",
          "reference_product_name": "polyurethane adhesive",
          "ecoinvent_row": 14055,
          "ecoinvent_geography": "GLO",
          "ecoinvent_matched": true
        },
        {
          "id": "pdf-1-5",
          "name": "Power Inverter & Solid-State VFD",
          "material": "electronics_vfd",
          "mass": 110,
          "unit": "kg",
          "ecoinvent_id": "ecoinvent_row_11483",
          "supplier": "Advantech Power Systems",
          "transport_km": 890,
          "module": "A1",
          "dataset": "market for electronics scrap [GLO]",
          "reference_product_name": "electronics scrap",
          "ecoinvent_row": 11483,
          "ecoinvent_geography": "GLO",
          "ecoinvent_matched": true
        },
        {
          "id": "pdf-1-6",
          "name": "Microchannel Subcooler Coil",
          "material": "aluminium_cast_alloy",
          "mass": 95,
          "unit": "kg",
          "ecoinvent_id": "ecoinvent_row_9452",
          "supplier": "Alloy Heat Exchangers",
          "transport_km": 350,
          "module": "A1",
          "dataset": "market for aluminium, cast alloy [GLO]",
          "reference_product_name": "aluminium, cast alloy",
          "ecoinvent_row": 9452,
          "ecoinvent_geography": "GLO",
          "ecoinvent_matched": true
        },
        {
          "id": "pdf-1-7",
          "name": "Refrigerant High-Pressure Piping",
          "material": "steel_stainless_304",
          "mass": 85,
          "unit": "kg",
          "ecoinvent_id": "ecoinvent_row_11757",
          "supplier": "Precision Alloy Tubing",
          "transport_km": 340,
          "module": "A1",
          "dataset": "market for forging, steel [GLO]",
          "reference_product_name": "forging, steel",
          "ecoinvent_row": 11757,
          "ecoinvent_geography": "GLO",
          "ecoinvent_matched": true
        },
        {
          "id": "pdf-1-8",
          "name": "Base Skid Frame & Mounts",
          "material": "steel_hot_rolled",
          "mass": 540,
          "unit": "kg",
          "ecoinvent_id": "ecoinvent_row_15528",
          "supplier": "ArcelorMittal Midwest",
          "transport_km": 260,
          "module": "A1",
          "dataset": "market for steel, low-alloyed, hot rolled [GLO]",
          "reference_product_name": "steel, low-alloyed, hot rolled",
          "ecoinvent_row": 15528,
          "ecoinvent_geography": "GLO",
          "ecoinvent_matched": true
        }
      ],
      "transport": [
        {
          "id": "a2-leg-1",
          "name": "Zurich Foundry Ltd (Genoa Port, Italy)",
          "mode": "Freight Train (Electric/Diesel)",
          "distance": 450,
          "dist": 450,
          "mass_kg": 2250,
          "emission_factor": 0.035,
          "ef": 0.035,
          "module": "A2"
        },
        {
          "id": "a2-leg-2",
          "name": "Mediterranean Shipping Co (Port of New York, USA)",
          "mode": "Transoceanic Container Ship",
          "distance": 6200,
          "dist": 6200,
          "mass_kg": 2250,
          "emission_factor": 0.0145,
          "ef": 0.0145,
          "module": "A2"
        },
        {
          "id": "a2-leg-3",
          "name": "Great Lakes Intermodal (Assembly Plant, Chicago IL)",
          "mode": "Freight Train (Electric/Diesel)",
          "distance": 900,
          "dist": 900,
          "mass_kg": 2250,
          "emission_factor": 0.035,
          "ef": 0.035,
          "module": "A2"
        },
        {
          "id": "a2-leg-4",
          "name": "Wieland Copper Mill (Rotterdam Port, Netherlands)",
          "mode": "Heavy Lorry >32t (EURO 6)",
          "distance": 620,
          "dist": 620,
          "mass_kg": 720,
          "emission_factor": 0.088,
          "ef": 0.088,
          "module": "A2"
        },
        {
          "id": "a2-leg-5",
          "name": "Atlantic Carrier Line (Montreal Port, Canada)",
          "mode": "Transoceanic Container Ship",
          "distance": 5850,
          "dist": 5850,
          "mass_kg": 720,
          "emission_factor": 0.0145,
          "ef": 0.0145,
          "module": "A2"
        },
        {
          "id": "a2-leg-6",
          "name": "Advantech Electronics (Long Beach Port, USA)",
          "mode": "Transoceanic Container Ship",
          "distance": 10800,
          "dist": 10800,
          "mass_kg": 110,
          "emission_factor": 0.0145,
          "ef": 0.0145,
          "module": "A2"
        },
        {
          "id": "a2-leg-7",
          "name": "US Pacific Trucking (Assembly Plant, Chicago IL)",
          "mode": "Heavy Lorry >32t (EURO 6)",
          "distance": 3250,
          "dist": 3250,
          "mass_kg": 110,
          "emission_factor": 0.088,
          "ef": 0.088,
          "module": "A2"
        },
        {
          "id": "a2-leg-8",
          "name": "ArcelorMittal Midwest (Assembly Plant, Chicago IL)",
          "mode": "Heavy Lorry >32t (EURO 6)",
          "distance": 85,
          "dist": 85,
          "mass_kg": 540,
          "emission_factor": 0.088,
          "ef": 0.088,
          "module": "A2"
        },
        {
          "id": "a2-leg-9",
          "name": "Armacell Polymer Systems (Assembly Plant, Chicago IL)",
          "mode": "Heavy Lorry >32t (EURO 6)",
          "distance": 1120,
          "dist": 1120,
          "mass_kg": 140,
          "emission_factor": 0.088,
          "ef": 0.088,
          "module": "A2"
        }
      ],
      "manufacturing": {
        "annual_facility_kwh": 34000,
        "natural_gas_mj": 0,
        "grid_region": "US_Average",
        "water_m3": 0
      },
      "installation": {
        "outbound_transport_km": 750,
        "transport_mode": "Heavy Lorry >32t (EURO 6)",
        "installation_energy_kwh": 350,
        "commissioning_refrigerant_loss_kg": 0.5,
        "rigging_crane_diesel_liters": 37.8
      },
      "maintenance_b2": {
        "consumable_mass_kg": 25,
        "provider_id": "ecoinvent_lubricating_oil_glo"
      },
      "repair_b3": {
        "repair_events_per_rsl": 0,
        "replaced_part_name": "",
        "part_mass_kg": 0,
        "material_type": "",
        "provider_id": "ecoinvent_steel_hot_rolled_glo"
      },
      "replacement_b4": {
        "esl_years": 25
      },
      "refurbishment_b5": {
        "refurbishment_events_per_rsl": 0,
        "material_name": "",
        "mass_kg": 0,
        "provider_id": "ecoinvent_copper_tube_wire_glo"
      },
      "operational": {
        "refrigerant_type": "R134A",
        "refrigerant_charge_kg": 45,
        "annual_leak_rate_percent": 2,
        "fugitive_operational_leak_rate": 0,
        "efficiency_kw_per_ton": 0.54,
        "capacity_rt": 500,
        "target_cities": [],
        "cooling_tower_water_m3_yr": 120,
        "scheduled_maintenance_kwh_yr": 0,
        "major_component_replacement_year": 15,
        "iplv_kw_per_ton": 0.435
      },
      "end_of_life": {
        "recycling_rate_percent": 92.4,
        "landfill_rate_percent": 4.5,
        "incineration_rate_percent": 3.1,
        "decommissioning_energy_kwh": 120,
        "waste_transport_km": 100
      },
      "circularity_d": {
        "steel_scrap_recovery_rate": 95,
        "copper_scrap_recovery_rate": 96,
        "aluminium_recovery_rate": 90,
        "refrigerant_reclamation_rate": 92,
        "net_avoided_burden_gwp_kg": -3210
      },
      "project_info": {
        "product_name": "Carrier AquaEdge 19DV Centrifugal Chiller",
        "manufacturer_name": "Declared Manufacturer",
        "functional_unit": "1 unit over 25 years reference service life (500.0 RT)",
        "declared_unit": "1 piece",
        "pcr_ref": "UL 10010-4 Part B & EN 15804+A2",
        "geography": "Global",
        "lifespan_years": 25
      }
    },
    "methodology": "ef31"
  },
  "extracted_ef_values": {
    "ecoinvent_diesel_burned_building_machine_glo": {
      "matched_activity_name": "diesel, burned in building machine",
      "matched_geography": "GLO",
      "match_confidence": "keyword (1 of 2 candidates)",
      "selected_methodology": "ef31",
      "values": {
        "EF v3.1 | acidification | accumulated exceedance (AE) [mol H+-Eq]": 0.0008990032175829071,
        "EF v3.1 | climate change | global warming potential (GWP100) [kg CO2-Eq]": 0.1006596082705705,
        "EF v3.1 | climate change: biogenic | global warming potential (GWP100) [kg CO2-Eq]": 1.006613289742308e-05,
        "EF v3.1 | climate change: fossil | global warming potential (GWP100) [kg CO2-Eq]": 0.1006393724831878,
        "EF v3.1 | climate change: land use and land use change | global warming potential (GWP100) [kg CO2-Eq]": 1.016965448526371e-05,
        "EF v3.1 | ecotoxicity: freshwater | comparative toxic unit for ecosystems (CTUe) [CTUe]": 0.1325251543172988,
        "EF v3.1 | ecotoxicity: freshwater, inorganics | comparative toxic unit for ecosystems (CTUe) [CTUe]": 0.119341530258097,
        "EF v3.1 | ecotoxicity: freshwater, organics | comparative toxic unit for ecosystems (CTUe) [CTUe]": 0.01318362405920172,
        "EF v3.1 | energy resources: non-renewable | abiotic depletion potential (ADP): fossil fuels [MJ, net calorific value]": 1.305190913934539,
        "EF v3.1 | eutrophication: freshwater | fraction of nutrients reaching freshwater end compartment (P) [kg P-Eq]": 3.231877988363177e-06,
        "EF v3.1 | eutrophication: marine | fraction of nutrients reaching marine end compartment (N) [kg N-Eq]": 0.0004212302871266372,
        "EF v3.1 | eutrophication: terrestrial | accumulated exceedance (AE) [mol N-Eq]": 0.004606094035841191,
        "EF v3.1 | human toxicity: carcinogenic | comparative toxic unit for human (CTUh) [CTUh]": 9.663046163680363e-12,
        "EF v3.1 | human toxicity: carcinogenic, inorganics | comparative toxic unit for human (CTUh) [CTUh]": 2.585444770802169e-12,
        "EF v3.1 | human toxicity: carcinogenic, organics | comparative toxic unit for human (CTUh) [CTUh]": 7.077601392878193e-12,
        "EF v3.1 | human toxicity: non-carcinogenic | comparative toxic unit for human (CTUh) [CTUh]": 1.721428660889974e-10,
        "EF v3.1 | human toxicity: non-carcinogenic, inorganics | comparative toxic unit for human (CTUh) [CTUh]": 1.44525879899594e-10,
        "EF v3.1 | human toxicity: non-carcinogenic, organics | comparative toxic unit for human (CTUh) [CTUh]": 2.761698618940329e-11,
        "EF v3.1 | ionising radiation: human health | human exposure efficiency relative to u235 [kBq U235-Eq]": 0.0005461534835623221,
        "EF v3.1 | land use | soil quality index [dimensionless]": 0.09038403299690947,
        "EF v3.1 | material resources: metals/minerals | abiotic depletion potential (ADP): elements (ultimate reserves) [kg Sb-Eq]": 3.740083879234519e-08,
        "EF v3.1 | ozone depletion | ozone depletion potential (ODP) [kg CFC-11-Eq]": 1.547590514595955e-09,
        "EF v3.1 | particulate matter formation | impact on human health [disease incidence]": 2.569240191303791e-08,
        "EF v3.1 | photochemical oxidant formation: human health | tropospheric ozone concentration increase [kg NMVOC-Eq]": 0.001381791867328339,
        "EF v3.1 | water use | user deprivation potential (deprivation-weighted water consumption) [m3 world Eq deprived]": 0.003273571451445218
      }
    },
    "ecoinvent_diesel_dismantling_glo": {
      "matched_activity_name": "chipper production, mobile, diesel",
      "matched_geography": "GLO",
      "match_confidence": "keyword (1 of 445 candidates)",
      "selected_methodology": "ef31",
      "values": {
        "EF v3.1 | acidification | accumulated exceedance (AE) [mol H+-Eq]": 1161.388443034718,
        "EF v3.1 | climate change | global warming potential (GWP100) [kg CO2-Eq]": 259220.222916975,
        "EF v3.1 | climate change: biogenic | global warming potential (GWP100) [kg CO2-Eq]": 272.361605188492,
        "EF v3.1 | climate change: fossil | global warming potential (GWP100) [kg CO2-Eq]": 258666.629318359,
        "EF v3.1 | climate change: land use and land use change | global warming potential (GWP100) [kg CO2-Eq]": 281.231993427513,
        "EF v3.1 | ecotoxicity: freshwater | comparative toxic unit for ecosystems (CTUe) [CTUe]": 1698182.631742193,
        "EF v3.1 | ecotoxicity: freshwater, inorganics | comparative toxic unit for ecosystems (CTUe) [CTUe]": 1661320.970023484,
        "EF v3.1 | ecotoxicity: freshwater, organics | comparative toxic unit for ecosystems (CTUe) [CTUe]": 36861.66171870985,
        "EF v3.1 | energy resources: non-renewable | abiotic depletion potential (ADP): fossil fuels [MJ, net calorific value]": 3100071.347393767,
        "EF v3.1 | eutrophication: freshwater | fraction of nutrients reaching freshwater end compartment (P) [kg P-Eq]": 138.428337689944,
        "EF v3.1 | eutrophication: marine | fraction of nutrients reaching marine end compartment (N) [kg N-Eq]": 250.4127849522965,
        "EF v3.1 | eutrophication: terrestrial | accumulated exceedance (AE) [mol N-Eq]": 2555.361276859482,
        "EF v3.1 | human toxicity: carcinogenic | comparative toxic unit for human (CTUh) [CTUh]": 0.0001817719370602114,
        "EF v3.1 | human toxicity: carcinogenic, inorganics | comparative toxic unit for human (CTUh) [CTUh]": 5.541891794840763e-05,
        "EF v3.1 | human toxicity: carcinogenic, organics | comparative toxic unit for human (CTUh) [CTUh]": 0.0001263530191118036,
        "EF v3.1 | human toxicity: non-carcinogenic | comparative toxic unit for human (CTUh) [CTUh]": 0.004333836493563533,
        "EF v3.1 | human toxicity: non-carcinogenic, inorganics | comparative toxic unit for human (CTUh) [CTUh]": 0.004209214837964003,
        "EF v3.1 | human toxicity: non-carcinogenic, organics | comparative toxic unit for human (CTUh) [CTUh]": 0.0001246216555995336,
        "EF v3.1 | ionising radiation: human health | human exposure efficiency relative to u235 [kBq U235-Eq]": 16228.80164526763,
        "EF v3.1 | land use | soil quality index [dimensionless]": 826052.1375894299,
        "EF v3.1 | material resources: metals/minerals | abiotic depletion potential (ADP): elements (ultimate reserves) [kg Sb-Eq]": 4.054334639899972,
        "EF v3.1 | ozone depletion | ozone depletion potential (ODP) [kg CFC-11-Eq]": 0.002425223511803635,
        "EF v3.1 | particulate matter formation | impact on human health [disease incidence]": 0.01983740112870816,
        "EF v3.1 | photochemical oxidant formation: human health | tropospheric ozone concentration increase [kg NMVOC-Eq]": 844.6442173083177,
        "EF v3.1 | water use | user deprivation potential (deprivation-weighted water consumption) [m3 world Eq deprived]": 82169.10331064301
      }
    },
    "ecoinvent_elec_ae": {
      "matched_activity_name": "electricity, high voltage, import from AE",
      "matched_geography": "SA",
      "match_confidence": "keyword (1 of 14 candidates)",
      "selected_methodology": "ef31",
      "values": {
        "EF v3.1 | acidification | accumulated exceedance (AE) [mol H+-Eq]": 0.0008143689070637498,
        "EF v3.1 | climate change | global warming potential (GWP100) [kg CO2-Eq]": 0.532550418415351,
        "EF v3.1 | climate change: biogenic | global warming potential (GWP100) [kg CO2-Eq]": 4.564223515933844e-05,
        "EF v3.1 | climate change: fossil | global warming potential (GWP100) [kg CO2-Eq]": 0.5324723748982336,
        "EF v3.1 | climate change: land use and land use change | global warming potential (GWP100) [kg CO2-Eq]": 3.240128195787749e-05,
        "EF v3.1 | ecotoxicity: freshwater | comparative toxic unit for ecosystems (CTUe) [CTUe]": 0.537937479254701,
        "EF v3.1 | ecotoxicity: freshwater, inorganics | comparative toxic unit for ecosystems (CTUe) [CTUe]": 0.4873889294265925,
        "EF v3.1 | ecotoxicity: freshwater, organics | comparative toxic unit for ecosystems (CTUe) [CTUe]": 0.05054854982810859,
        "EF v3.1 | energy resources: non-renewable | abiotic depletion potential (ADP): fossil fuels [MJ, net calorific value]": 10.29102128175109,
        "EF v3.1 | eutrophication: freshwater | fraction of nutrients reaching freshwater end compartment (P) [kg P-Eq]": 2.250288321167098e-05,
        "EF v3.1 | eutrophication: marine | fraction of nutrients reaching marine end compartment (N) [kg N-Eq]": 0.0002204743674114944,
        "EF v3.1 | eutrophication: terrestrial | accumulated exceedance (AE) [mol N-Eq]": 0.002250439619866153,
        "EF v3.1 | human toxicity: carcinogenic | comparative toxic unit for human (CTUh) [CTUh]": 4.092682511295035e-11,
        "EF v3.1 | human toxicity: carcinogenic, inorganics | comparative toxic unit for human (CTUh) [CTUh]": 8.692189862748175e-12,
        "EF v3.1 | human toxicity: carcinogenic, organics | comparative toxic unit for human (CTUh) [CTUh]": 3.223463525020216e-11,
        "EF v3.1 | human toxicity: non-carcinogenic | comparative toxic unit for human (CTUh) [CTUh]": 9.15148150596627e-10,
        "EF v3.1 | human toxicity: non-carcinogenic, inorganics | comparative toxic unit for human (CTUh) [CTUh]": 7.918544564120659e-10,
        "EF v3.1 | human toxicity: non-carcinogenic, organics | comparative toxic unit for human (CTUh) [CTUh]": 1.232936941845629e-10,
        "EF v3.1 | ionising radiation: human health | human exposure efficiency relative to u235 [kBq U235-Eq]": 0.1034724517851093,
        "EF v3.1 | land use | soil quality index [dimensionless]": 0.184242111359898,
        "EF v3.1 | material resources: metals/minerals | abiotic depletion potential (ADP): elements (ultimate reserves) [kg Sb-Eq]": 3.181487006512287e-07,
        "EF v3.1 | ozone depletion | ozone depletion potential (ODP) [kg CFC-11-Eq]": 1.185279531985281e-08,
        "EF v3.1 | particulate matter formation | impact on human health [disease incidence]": 2.940923953579584e-09,
        "EF v3.1 | photochemical oxidant formation: human health | tropospheric ozone concentration increase [kg NMVOC-Eq]": 0.001413958358909779,
        "EF v3.1 | water use | user deprivation potential (deprivation-weighted water consumption) [m3 world Eq deprived]": 0.05809457111185774
      }
    },
    "ecoinvent_elec_de": {
      "matched_activity_name": "electricity production, deep geothermal",
      "matched_geography": "DE",
      "match_confidence": "keyword (1 of 55 candidates)",
      "selected_methodology": "ef31",
      "values": {
        "EF v3.1 | acidification | accumulated exceedance (AE) [mol H+-Eq]": 0.0003423907244437862,
        "EF v3.1 | climate change | global warming potential (GWP100) [kg CO2-Eq]": 0.06929879682757782,
        "EF v3.1 | climate change: biogenic | global warming potential (GWP100) [kg CO2-Eq]": 9.310794401122473e-05,
        "EF v3.1 | climate change: fossil | global warming potential (GWP100) [kg CO2-Eq]": 0.06910394985525552,
        "EF v3.1 | climate change: land use and land use change | global warming potential (GWP100) [kg CO2-Eq]": 0.0001017390283110599,
        "EF v3.1 | ecotoxicity: freshwater | comparative toxic unit for ecosystems (CTUe) [CTUe]": 0.5680758453082888,
        "EF v3.1 | ecotoxicity: freshwater, inorganics | comparative toxic unit for ecosystems (CTUe) [CTUe]": 0.5616416220087681,
        "EF v3.1 | ecotoxicity: freshwater, organics | comparative toxic unit for ecosystems (CTUe) [CTUe]": 0.006434223299520515,
        "EF v3.1 | energy resources: non-renewable | abiotic depletion potential (ADP): fossil fuels [MJ, net calorific value]": 0.8413728705806833,
        "EF v3.1 | eutrophication: freshwater | fraction of nutrients reaching freshwater end compartment (P) [kg P-Eq]": 3.670511040896688e-05,
        "EF v3.1 | eutrophication: marine | fraction of nutrients reaching marine end compartment (N) [kg N-Eq]": 7.282185344684724e-05,
        "EF v3.1 | eutrophication: terrestrial | accumulated exceedance (AE) [mol N-Eq]": 0.0007339967577177946,
        "EF v3.1 | human toxicity: carcinogenic | comparative toxic unit for human (CTUh) [CTUh]": 2.731155511371121e-11,
        "EF v3.1 | human toxicity: carcinogenic, inorganics | comparative toxic unit for human (CTUh) [CTUh]": 7.586112281222163e-12,
        "EF v3.1 | human toxicity: carcinogenic, organics | comparative toxic unit for human (CTUh) [CTUh]": 1.972544283248905e-11,
        "EF v3.1 | human toxicity: non-carcinogenic | comparative toxic unit for human (CTUh) [CTUh]": 7.242832636628451e-10,
        "EF v3.1 | human toxicity: non-carcinogenic, inorganics | comparative toxic unit for human (CTUh) [CTUh]": 7.062706304886898e-10,
        "EF v3.1 | human toxicity: non-carcinogenic, organics | comparative toxic unit for human (CTUh) [CTUh]": 1.801263317415651e-11,
        "EF v3.1 | ionising radiation: human health | human exposure efficiency relative to u235 [kBq U235-Eq]": 0.006300658346208351,
        "EF v3.1 | land use | soil quality index [dimensionless]": 0.2781987958249374,
        "EF v3.1 | material resources: metals/minerals | abiotic depletion potential (ADP): elements (ultimate reserves) [kg Sb-Eq]": 1.810694462900144e-07,
        "EF v3.1 | ozone depletion | ozone depletion potential (ODP) [kg CFC-11-Eq]": 9.38198528390253e-10,
        "EF v3.1 | particulate matter formation | impact on human health [disease incidence]": 3.944365325682737e-09,
        "EF v3.1 | photochemical oxidant formation: human health | tropospheric ozone concentration increase [kg NMVOC-Eq]": 0.0002211556163862941,
        "EF v3.1 | water use | user deprivation potential (deprivation-weighted water consumption) [m3 world Eq deprived]": 0.01845807255481025
      }
    },
    "ecoinvent_elec_mv_us": {
      "matched_activity_name": "cadmium sludge from zinc electrolysis stockpiling",
      "matched_geography": "US",
      "match_confidence": "keyword (1 of 22 candidates)",
      "selected_methodology": "ef31",
      "values": {
        "EF v3.1 | acidification | accumulated exceedance (AE) [mol H+-Eq]": 0.01288047140644808,
        "EF v3.1 | climate change | global warming potential (GWP100) [kg CO2-Eq]": 1.282040309610317,
        "EF v3.1 | climate change: biogenic | global warming potential (GWP100) [kg CO2-Eq]": 0.007955163191450124,
        "EF v3.1 | climate change: fossil | global warming potential (GWP100) [kg CO2-Eq]": 1.268130254685141,
        "EF v3.1 | climate change: land use and land use change | global warming potential (GWP100) [kg CO2-Eq]": 0.005954891733725221,
        "EF v3.1 | ecotoxicity: freshwater | comparative toxic unit for ecosystems (CTUe) [CTUe]": 237.2005053069147,
        "EF v3.1 | ecotoxicity: freshwater, inorganics | comparative toxic unit for ecosystems (CTUe) [CTUe]": 237.0666242563236,
        "EF v3.1 | ecotoxicity: freshwater, organics | comparative toxic unit for ecosystems (CTUe) [CTUe]": 0.1338810505910669,
        "EF v3.1 | energy resources: non-renewable | abiotic depletion potential (ADP): fossil fuels [MJ, net calorific value]": 19.46769699128178,
        "EF v3.1 | eutrophication: freshwater | fraction of nutrients reaching freshwater end compartment (P) [kg P-Eq]": 0.001858534921893695,
        "EF v3.1 | eutrophication: marine | fraction of nutrients reaching marine end compartment (N) [kg N-Eq]": 0.003143518617408705,
        "EF v3.1 | eutrophication: terrestrial | accumulated exceedance (AE) [mol N-Eq]": 0.03363472183507096,
        "EF v3.1 | human toxicity: carcinogenic | comparative toxic unit for human (CTUh) [CTUh]": 7.118412475383828e-09,
        "EF v3.1 | human toxicity: carcinogenic, inorganics | comparative toxic unit for human (CTUh) [CTUh]": 6.948445952904258e-09,
        "EF v3.1 | human toxicity: carcinogenic, organics | comparative toxic unit for human (CTUh) [CTUh]": 1.699665224795666e-10,
        "EF v3.1 | human toxicity: non-carcinogenic | comparative toxic unit for human (CTUh) [CTUh]": 1.782650588789809e-07,
        "EF v3.1 | human toxicity: non-carcinogenic, inorganics | comparative toxic unit for human (CTUh) [CTUh]": 1.731319775844884e-07,
        "EF v3.1 | human toxicity: non-carcinogenic, organics | comparative toxic unit for human (CTUh) [CTUh]": 5.133081294492349e-09,
        "EF v3.1 | ionising radiation: human health | human exposure efficiency relative to u235 [kBq U235-Eq]": 0.2975185961579512,
        "EF v3.1 | land use | soil quality index [dimensionless]": 11.20229811440402,
        "EF v3.1 | material resources: metals/minerals | abiotic depletion potential (ADP): elements (ultimate reserves) [kg Sb-Eq]": 0.0009129532533534276,
        "EF v3.1 | ozone depletion | ozone depletion potential (ODP) [kg CFC-11-Eq]": 1.965113558728618e-08,
        "EF v3.1 | particulate matter formation | impact on human health [disease incidence]": 6.8884765365508e-08,
        "EF v3.1 | photochemical oxidant formation: human health | tropospheric ozone concentration increase [kg NMVOC-Eq]": 0.008804375665365866,
        "EF v3.1 | water use | user deprivation potential (deprivation-weighted water consumption) [m3 world Eq deprived]": 1.803242077433189
      }
    },
    "ecoinvent_elec_tx": {
      "matched_activity_name": "BTX production, from pyrolysis gas, average",
      "matched_geography": "RoW",
      "match_confidence": "keyword (1 of 4563 candidates)",
      "selected_methodology": "ef31",
      "values": {
        "EF v3.1 | acidification | accumulated exceedance (AE) [mol H+-Eq]": 0.007005014280917295,
        "EF v3.1 | climate change | global warming potential (GWP100) [kg CO2-Eq]": 2.094180541717069,
        "EF v3.1 | climate change: biogenic | global warming potential (GWP100) [kg CO2-Eq]": 0.0008971937027153093,
        "EF v3.1 | climate change: fossil | global warming potential (GWP100) [kg CO2-Eq]": 2.092549903349286,
        "EF v3.1 | climate change: land use and land use change | global warming potential (GWP100) [kg CO2-Eq]": 0.0007334446650677486,
        "EF v3.1 | ecotoxicity: freshwater | comparative toxic unit for ecosystems (CTUe) [CTUe]": 8.670892819537507,
        "EF v3.1 | ecotoxicity: freshwater, inorganics | comparative toxic unit for ecosystems (CTUe) [CTUe]": 7.925531460031578,
        "EF v3.1 | ecotoxicity: freshwater, organics | comparative toxic unit for ecosystems (CTUe) [CTUe]": 0.7453613595059395,
        "EF v3.1 | energy resources: non-renewable | abiotic depletion potential (ADP): fossil fuels [MJ, net calorific value]": 75.68714969369408,
        "EF v3.1 | eutrophication: freshwater | fraction of nutrients reaching freshwater end compartment (P) [kg P-Eq]": 0.0002210452671549384,
        "EF v3.1 | eutrophication: marine | fraction of nutrients reaching marine end compartment (N) [kg N-Eq]": 0.001394416056929574,
        "EF v3.1 | eutrophication: terrestrial | accumulated exceedance (AE) [mol N-Eq]": 0.01444115556013529,
        "EF v3.1 | human toxicity: carcinogenic | comparative toxic unit for human (CTUh) [CTUh]": 3.345706265964019e-10,
        "EF v3.1 | human toxicity: carcinogenic, inorganics | comparative toxic unit for human (CTUh) [CTUh]": 1.573409325940652e-10,
        "EF v3.1 | human toxicity: carcinogenic, organics | comparative toxic unit for human (CTUh) [CTUh]": 1.772296940023366e-10,
        "EF v3.1 | human toxicity: non-carcinogenic | comparative toxic unit for human (CTUh) [CTUh]": 1.352196739190723e-08,
        "EF v3.1 | human toxicity: non-carcinogenic, inorganics | comparative toxic unit for human (CTUh) [CTUh]": 1.224699319025207e-08,
        "EF v3.1 | human toxicity: non-carcinogenic, organics | comparative toxic unit for human (CTUh) [CTUh]": 1.274974201655163e-09,
        "EF v3.1 | ionising radiation: human health | human exposure efficiency relative to u235 [kBq U235-Eq]": 0.03981394890484413,
        "EF v3.1 | land use | soil quality index [dimensionless]": 5.212473531147947,
        "EF v3.1 | material resources: metals/minerals | abiotic depletion potential (ADP): elements (ultimate reserves) [kg Sb-Eq]": 1.017535254432217e-05,
        "EF v3.1 | ozone depletion | ozone depletion potential (ODP) [kg CFC-11-Eq]": 8.716043435885687e-08,
        "EF v3.1 | particulate matter formation | impact on human health [disease incidence]": 5.804064533252954e-08,
        "EF v3.1 | photochemical oxidant formation: human health | tropospheric ozone concentration increase [kg NMVOC-Eq]": 0.01184262880138768,
        "EF v3.1 | water use | user deprivation potential (deprivation-weighted water consumption) [m3 world Eq deprived]": 0.3227317470720872
      }
    },
    "ecoinvent_lubricating_oil_glo": {
      "matched_activity_name": "lubricating oil production",
      "matched_geography": "RoW",
      "match_confidence": "keyword (1 of 4 candidates)",
      "selected_methodology": "ef31",
      "values": {
        "EF v3.1 | acidification | accumulated exceedance (AE) [mol H+-Eq]": 0.007709523132801899,
        "EF v3.1 | climate change | global warming potential (GWP100) [kg CO2-Eq]": 1.699958012410375,
        "EF v3.1 | climate change: biogenic | global warming potential (GWP100) [kg CO2-Eq]": 0.001696448684812329,
        "EF v3.1 | climate change: fossil | global warming potential (GWP100) [kg CO2-Eq]": 1.696928360585128,
        "EF v3.1 | climate change: land use and land use change | global warming potential (GWP100) [kg CO2-Eq]": 0.001333203140434814,
        "EF v3.1 | ecotoxicity: freshwater | comparative toxic unit for ecosystems (CTUe) [CTUe]": 10.20361396753049,
        "EF v3.1 | ecotoxicity: freshwater, inorganics | comparative toxic unit for ecosystems (CTUe) [CTUe]": 9.3525850210745,
        "EF v3.1 | ecotoxicity: freshwater, organics | comparative toxic unit for ecosystems (CTUe) [CTUe]": 0.8510289464559854,
        "EF v3.1 | energy resources: non-renewable | abiotic depletion potential (ADP): fossil fuels [MJ, net calorific value]": 63.14939266879649,
        "EF v3.1 | eutrophication: freshwater | fraction of nutrients reaching freshwater end compartment (P) [kg P-Eq]": 0.0003672162606996572,
        "EF v3.1 | eutrophication: marine | fraction of nutrients reaching marine end compartment (N) [kg N-Eq]": 0.001447473201881779,
        "EF v3.1 | eutrophication: terrestrial | accumulated exceedance (AE) [mol N-Eq]": 0.01498380513572746,
        "EF v3.1 | human toxicity: carcinogenic | comparative toxic unit for human (CTUh) [CTUh]": 3.932937539073314e-10,
        "EF v3.1 | human toxicity: carcinogenic, inorganics | comparative toxic unit for human (CTUh) [CTUh]": 2.018242082274763e-10,
        "EF v3.1 | human toxicity: carcinogenic, organics | comparative toxic unit for human (CTUh) [CTUh]": 1.914695456798551e-10,
        "EF v3.1 | human toxicity: non-carcinogenic | comparative toxic unit for human (CTUh) [CTUh]": 1.802596010260655e-08,
        "EF v3.1 | human toxicity: non-carcinogenic, inorganics | comparative toxic unit for human (CTUh) [CTUh]": 1.446815225682597e-08,
        "EF v3.1 | human toxicity: non-carcinogenic, organics | comparative toxic unit for human (CTUh) [CTUh]": 3.557807845780615e-09,
        "EF v3.1 | ionising radiation: human health | human exposure efficiency relative to u235 [kBq U235-Eq]": 0.06899714425654603,
        "EF v3.1 | land use | soil quality index [dimensionless]": 6.115068648255371,
        "EF v3.1 | material resources: metals/minerals | abiotic depletion potential (ADP): elements (ultimate reserves) [kg Sb-Eq]": 1.383330968980312e-05,
        "EF v3.1 | ozone depletion | ozone depletion potential (ODP) [kg CFC-11-Eq]": 7.200270956408488e-08,
        "EF v3.1 | particulate matter formation | impact on human health [disease incidence]": 7.958430700730498e-08,
        "EF v3.1 | photochemical oxidant formation: human health | tropospheric ozone concentration increase [kg NMVOC-Eq]": 0.03151667465089646,
        "EF v3.1 | water use | user deprivation potential (deprivation-weighted water consumption) [m3 world Eq deprived]": 0.377354310603073
      }
    },
    "ecoinvent_row_10657": {
      "matched_activity_name": "market for copper slag",
      "matched_geography": "GLO",
      "match_confidence": "row_index (row 10657)",
      "selected_methodology": "ef31",
      "values": {
        "EF v3.1 | acidification | accumulated exceedance (AE) [mol H+-Eq]": 0.0001023674175810036,
        "EF v3.1 | climate change | global warming potential (GWP100) [kg CO2-Eq]": 0.01903800570665727,
        "EF v3.1 | climate change: biogenic | global warming potential (GWP100) [kg CO2-Eq]": 5.587416209296461e-06,
        "EF v3.1 | climate change: fossil | global warming potential (GWP100) [kg CO2-Eq]": 0.01898789557653824,
        "EF v3.1 | climate change: land use and land use change | global warming potential (GWP100) [kg CO2-Eq]": 4.452271390973959e-05,
        "EF v3.1 | ecotoxicity: freshwater | comparative toxic unit for ecosystems (CTUe) [CTUe]": 0.2743055936925144,
        "EF v3.1 | ecotoxicity: freshwater, inorganics | comparative toxic unit for ecosystems (CTUe) [CTUe]": 0.2681946331855622,
        "EF v3.1 | ecotoxicity: freshwater, organics | comparative toxic unit for ecosystems (CTUe) [CTUe]": 0.00611096050695237,
        "EF v3.1 | energy resources: non-renewable | abiotic depletion potential (ADP): fossil fuels [MJ, net calorific value]": 0.3182060350036132,
        "EF v3.1 | eutrophication: freshwater | fraction of nutrients reaching freshwater end compartment (P) [kg P-Eq]": 2.055062215327943e-06,
        "EF v3.1 | eutrophication: marine | fraction of nutrients reaching marine end compartment (N) [kg N-Eq]": 3.97694526135736e-05,
        "EF v3.1 | eutrophication: terrestrial | accumulated exceedance (AE) [mol N-Eq]": 0.0004293256150162811,
        "EF v3.1 | human toxicity: carcinogenic | comparative toxic unit for human (CTUh) [CTUh]": 3.796665670005462e-10,
        "EF v3.1 | human toxicity: carcinogenic, inorganics | comparative toxic unit for human (CTUh) [CTUh]": 3.766447209478858e-10,
        "EF v3.1 | human toxicity: carcinogenic, organics | comparative toxic unit for human (CTUh) [CTUh]": 3.021846052660329e-12,
        "EF v3.1 | human toxicity: non-carcinogenic | comparative toxic unit for human (CTUh) [CTUh]": 1.568073759295228e-08,
        "EF v3.1 | human toxicity: non-carcinogenic, inorganics | comparative toxic unit for human (CTUh) [CTUh]": 1.565940668240591e-08,
        "EF v3.1 | human toxicity: non-carcinogenic, organics | comparative toxic unit for human (CTUh) [CTUh]": 2.133091054641719e-11,
        "EF v3.1 | ionising radiation: human health | human exposure efficiency relative to u235 [kBq U235-Eq]": 0.0002706352990488331,
        "EF v3.1 | land use | soil quality index [dimensionless]": 0.7771819514607539,
        "EF v3.1 | material resources: metals/minerals | abiotic depletion potential (ADP): elements (ultimate reserves) [kg Sb-Eq]": 5.588180814187136e-08,
        "EF v3.1 | ozone depletion | ozone depletion potential (ODP) [kg CFC-11-Eq]": 3.86350221015672e-10,
        "EF v3.1 | particulate matter formation | impact on human health [disease incidence]": 2.264799468605613e-09,
        "EF v3.1 | photochemical oxidant formation: human health | tropospheric ozone concentration increase [kg NMVOC-Eq]": 0.000148842168575174,
        "EF v3.1 | water use | user deprivation potential (deprivation-weighted water consumption) [m3 world Eq deprived]": 0.0098263742314527
      }
    },
    "ecoinvent_row_10882": {
      "matched_activity_name": "market for electric kettle",
      "matched_geography": "GLO",
      "match_confidence": "row_index (row 10882)",
      "selected_methodology": "ef31",
      "values": {
        "EF v3.1 | acidification | accumulated exceedance (AE) [mol H+-Eq]": 0.1416820093209528,
        "EF v3.1 | climate change | global warming potential (GWP100) [kg CO2-Eq]": 6.962374292469472,
        "EF v3.1 | climate change: biogenic | global warming potential (GWP100) [kg CO2-Eq]": 0.009476596388055685,
        "EF v3.1 | climate change: fossil | global warming potential (GWP100) [kg CO2-Eq]": 6.945219973762884,
        "EF v3.1 | climate change: land use and land use change | global warming potential (GWP100) [kg CO2-Eq]": 0.007677722318532584,
        "EF v3.1 | ecotoxicity: freshwater | comparative toxic unit for ecosystems (CTUe) [CTUe]": 105.8066764194711,
        "EF v3.1 | ecotoxicity: freshwater, inorganics | comparative toxic unit for ecosystems (CTUe) [CTUe]": 104.3389799168754,
        "EF v3.1 | ecotoxicity: freshwater, organics | comparative toxic unit for ecosystems (CTUe) [CTUe]": 1.467696502595445,
        "EF v3.1 | energy resources: non-renewable | abiotic depletion potential (ADP): fossil fuels [MJ, net calorific value]": 115.6918655302636,
        "EF v3.1 | eutrophication: freshwater | fraction of nutrients reaching freshwater end compartment (P) [kg P-Eq]": 0.003915734649202627,
        "EF v3.1 | eutrophication: marine | fraction of nutrients reaching marine end compartment (N) [kg N-Eq]": 0.007738363899729644,
        "EF v3.1 | eutrophication: terrestrial | accumulated exceedance (AE) [mol N-Eq]": 0.08226385715214936,
        "EF v3.1 | human toxicity: carcinogenic | comparative toxic unit for human (CTUh) [CTUh]": 2.096118733512706e-08,
        "EF v3.1 | human toxicity: carcinogenic, inorganics | comparative toxic unit for human (CTUh) [CTUh]": 4.948775090340195e-09,
        "EF v3.1 | human toxicity: carcinogenic, organics | comparative toxic unit for human (CTUh) [CTUh]": 1.601241224478687e-08,
        "EF v3.1 | human toxicity: non-carcinogenic | comparative toxic unit for human (CTUh) [CTUh]": 2.565751576188472e-07,
        "EF v3.1 | human toxicity: non-carcinogenic, inorganics | comparative toxic unit for human (CTUh) [CTUh]": 2.42108339891639e-07,
        "EF v3.1 | human toxicity: non-carcinogenic, organics | comparative toxic unit for human (CTUh) [CTUh]": 1.446681772720841e-08,
        "EF v3.1 | ionising radiation: human health | human exposure efficiency relative to u235 [kBq U235-Eq]": 0.4524896133048148,
        "EF v3.1 | land use | soil quality index [dimensionless]": 34.80655223921012,
        "EF v3.1 | material resources: metals/minerals | abiotic depletion potential (ADP): elements (ultimate reserves) [kg Sb-Eq]": 0.0003885734853635786,
        "EF v3.1 | ozone depletion | ozone depletion potential (ODP) [kg CFC-11-Eq]": 2.055001276432738e-06,
        "EF v3.1 | particulate matter formation | impact on human health [disease incidence]": 8.680178930939334e-07,
        "EF v3.1 | photochemical oxidant formation: human health | tropospheric ozone concentration increase [kg NMVOC-Eq]": 0.03815117052864314,
        "EF v3.1 | water use | user deprivation potential (deprivation-weighted water consumption) [m3 world Eq deprived]": 6.986819594465186
      }
    },
    "ecoinvent_row_11483": {
      "matched_activity_name": "market for electronics scrap",
      "matched_geography": "GLO",
      "match_confidence": "row_index (row 11483)",
      "selected_methodology": "ef31",
      "values": {
        "EF v3.1 | acidification | accumulated exceedance (AE) [mol H+-Eq]": 0.0002351480893291133,
        "EF v3.1 | climate change | global warming potential (GWP100) [kg CO2-Eq]": 0.03905341502694284,
        "EF v3.1 | climate change: biogenic | global warming potential (GWP100) [kg CO2-Eq]": 1.107771200244941e-05,
        "EF v3.1 | climate change: fossil | global warming potential (GWP100) [kg CO2-Eq]": 0.03893470803591439,
        "EF v3.1 | climate change: land use and land use change | global warming potential (GWP100) [kg CO2-Eq]": 0.0001076292790259942,
        "EF v3.1 | ecotoxicity: freshwater | comparative toxic unit for ecosystems (CTUe) [CTUe]": 0.1221395208808846,
        "EF v3.1 | ecotoxicity: freshwater, inorganics | comparative toxic unit for ecosystems (CTUe) [CTUe]": 0.1096335491024464,
        "EF v3.1 | ecotoxicity: freshwater, organics | comparative toxic unit for ecosystems (CTUe) [CTUe]": 0.01250597177843831,
        "EF v3.1 | energy resources: non-renewable | abiotic depletion potential (ADP): fossil fuels [MJ, net calorific value]": 0.5329001496018348,
        "EF v3.1 | eutrophication: freshwater | fraction of nutrients reaching freshwater end compartment (P) [kg P-Eq]": 4.58411581960889e-06,
        "EF v3.1 | eutrophication: marine | fraction of nutrients reaching marine end compartment (N) [kg N-Eq]": 9.234432095527185e-05,
        "EF v3.1 | eutrophication: terrestrial | accumulated exceedance (AE) [mol N-Eq]": 0.0009991917517985188,
        "EF v3.1 | human toxicity: carcinogenic | comparative toxic unit for human (CTUh) [CTUh]": 8.933275263674984e-12,
        "EF v3.1 | human toxicity: carcinogenic, inorganics | comparative toxic unit for human (CTUh) [CTUh]": 2.822278176741944e-12,
        "EF v3.1 | human toxicity: carcinogenic, organics | comparative toxic unit for human (CTUh) [CTUh]": 6.110997086933038e-12,
        "EF v3.1 | human toxicity: non-carcinogenic | comparative toxic unit for human (CTUh) [CTUh]": 3.344364028408298e-10,
        "EF v3.1 | human toxicity: non-carcinogenic, inorganics | comparative toxic unit for human (CTUh) [CTUh]": 2.871753735927915e-10,
        "EF v3.1 | human toxicity: non-carcinogenic, organics | comparative toxic unit for human (CTUh) [CTUh]": 4.726102924803842e-11,
        "EF v3.1 | ionising radiation: human health | human exposure efficiency relative to u235 [kBq U235-Eq]": 0.0006033760131612219,
        "EF v3.1 | land use | soil quality index [dimensionless]": 0.3933792640775375,
        "EF v3.1 | material resources: metals/minerals | abiotic depletion potential (ADP): elements (ultimate reserves) [kg Sb-Eq]": 1.202998787735548e-07,
        "EF v3.1 | ozone depletion | ozone depletion potential (ODP) [kg CFC-11-Eq]": 6.184881952200202e-10,
        "EF v3.1 | particulate matter formation | impact on human health [disease incidence]": 3.843206323431404e-09,
        "EF v3.1 | photochemical oxidant formation: human health | tropospheric ozone concentration increase [kg NMVOC-Eq]": 0.0003171259836351294,
        "EF v3.1 | water use | user deprivation potential (deprivation-weighted water consumption) [m3 world Eq deprived]": 0.003399491660427854
      }
    },
    "ecoinvent_row_11757": {
      "matched_activity_name": "market for forging, steel",
      "matched_geography": "GLO",
      "match_confidence": "row_index (row 11757)",
      "selected_methodology": "ef31",
      "values": {
        "EF v3.1 | acidification | accumulated exceedance (AE) [mol H+-Eq]": 0.003841172715116979,
        "EF v3.1 | climate change | global warming potential (GWP100) [kg CO2-Eq]": 1.196290181775795,
        "EF v3.1 | climate change: biogenic | global warming potential (GWP100) [kg CO2-Eq]": 0.0008196075269220426,
        "EF v3.1 | climate change: fossil | global warming potential (GWP100) [kg CO2-Eq]": 1.194466816387519,
        "EF v3.1 | climate change: land use and land use change | global warming potential (GWP100) [kg CO2-Eq]": 0.001003757861353779,
        "EF v3.1 | ecotoxicity: freshwater | comparative toxic unit for ecosystems (CTUe) [CTUe]": 5.081903564261311,
        "EF v3.1 | ecotoxicity: freshwater, inorganics | comparative toxic unit for ecosystems (CTUe) [CTUe]": 4.907626744338034,
        "EF v3.1 | ecotoxicity: freshwater, organics | comparative toxic unit for ecosystems (CTUe) [CTUe]": 0.1742768199232815,
        "EF v3.1 | energy resources: non-renewable | abiotic depletion potential (ADP): fossil fuels [MJ, net calorific value]": 15.90186817719698,
        "EF v3.1 | eutrophication: freshwater | fraction of nutrients reaching freshwater end compartment (P) [kg P-Eq]": 0.0004262357449695497,
        "EF v3.1 | eutrophication: marine | fraction of nutrients reaching marine end compartment (N) [kg N-Eq]": 0.0009188103639027847,
        "EF v3.1 | eutrophication: terrestrial | accumulated exceedance (AE) [mol N-Eq]": 0.00938173325514639,
        "EF v3.1 | human toxicity: carcinogenic | comparative toxic unit for human (CTUh) [CTUh]": 6.32241293422903e-10,
        "EF v3.1 | human toxicity: carcinogenic, inorganics | comparative toxic unit for human (CTUh) [CTUh]": 1.65985219349447e-10,
        "EF v3.1 | human toxicity: carcinogenic, organics | comparative toxic unit for human (CTUh) [CTUh]": 4.662560740734561e-10,
        "EF v3.1 | human toxicity: non-carcinogenic | comparative toxic unit for human (CTUh) [CTUh]": 1.285395199388811e-08,
        "EF v3.1 | human toxicity: non-carcinogenic, inorganics | comparative toxic unit for human (CTUh) [CTUh]": 1.242064594345598e-08,
        "EF v3.1 | human toxicity: non-carcinogenic, organics | comparative toxic unit for human (CTUh) [CTUh]": 4.333060504321292e-10,
        "EF v3.1 | ionising radiation: human health | human exposure efficiency relative to u235 [kBq U235-Eq]": 0.050333629847049,
        "EF v3.1 | land use | soil quality index [dimensionless]": 2.573091326151144,
        "EF v3.1 | material resources: metals/minerals | abiotic depletion potential (ADP): elements (ultimate reserves) [kg Sb-Eq]": 5.615976018745503e-06,
        "EF v3.1 | ozone depletion | ozone depletion potential (ODP) [kg CFC-11-Eq]": 1.63879613380161e-08,
        "EF v3.1 | particulate matter formation | impact on human health [disease incidence]": 6.380871378301805e-08,
        "EF v3.1 | photochemical oxidant formation: human health | tropospheric ozone concentration increase [kg NMVOC-Eq]": 0.003404404491866399,
        "EF v3.1 | water use | user deprivation potential (deprivation-weighted water consumption) [m3 world Eq deprived]": 0.2828360480250945
      }
    },
    "ecoinvent_row_14055": {
      "matched_activity_name": "market for polyurethane adhesive",
      "matched_geography": "GLO",
      "match_confidence": "row_index (row 14055)",
      "selected_methodology": "ef31",
      "values": {
        "EF v3.1 | acidification | accumulated exceedance (AE) [mol H+-Eq]": 0.0221967506915827,
        "EF v3.1 | climate change | global warming potential (GWP100) [kg CO2-Eq]": 5.328351278133265,
        "EF v3.1 | climate change: biogenic | global warming potential (GWP100) [kg CO2-Eq]": 0.004218683621325334,
        "EF v3.1 | climate change: fossil | global warming potential (GWP100) [kg CO2-Eq]": 5.307752035043736,
        "EF v3.1 | climate change: land use and land use change | global warming potential (GWP100) [kg CO2-Eq]": 0.016380559468204,
        "EF v3.1 | ecotoxicity: freshwater | comparative toxic unit for ecosystems (CTUe) [CTUe]": 171.2638652385652,
        "EF v3.1 | ecotoxicity: freshwater, inorganics | comparative toxic unit for ecosystems (CTUe) [CTUe]": 158.7494646889272,
        "EF v3.1 | ecotoxicity: freshwater, organics | comparative toxic unit for ecosystems (CTUe) [CTUe]": 12.5144005496381,
        "EF v3.1 | energy resources: non-renewable | abiotic depletion potential (ADP): fossil fuels [MJ, net calorific value]": 98.23597394920596,
        "EF v3.1 | eutrophication: freshwater | fraction of nutrients reaching freshwater end compartment (P) [kg P-Eq]": 0.001420841566033044,
        "EF v3.1 | eutrophication: marine | fraction of nutrients reaching marine end compartment (N) [kg N-Eq]": 0.006731168894221163,
        "EF v3.1 | eutrophication: terrestrial | accumulated exceedance (AE) [mol N-Eq]": 0.05111534826455191,
        "EF v3.1 | human toxicity: carcinogenic | comparative toxic unit for human (CTUh) [CTUh]": 7.638860189896111e-09,
        "EF v3.1 | human toxicity: carcinogenic, inorganics | comparative toxic unit for human (CTUh) [CTUh]": 5.606433617695389e-10,
        "EF v3.1 | human toxicity: carcinogenic, organics | comparative toxic unit for human (CTUh) [CTUh]": 7.078216828126571e-09,
        "EF v3.1 | human toxicity: non-carcinogenic | comparative toxic unit for human (CTUh) [CTUh]": 5.184099427670556e-08,
        "EF v3.1 | human toxicity: non-carcinogenic, inorganics | comparative toxic unit for human (CTUh) [CTUh]": 4.723962270009369e-08,
        "EF v3.1 | human toxicity: non-carcinogenic, organics | comparative toxic unit for human (CTUh) [CTUh]": 4.601371576611867e-09,
        "EF v3.1 | ionising radiation: human health | human exposure efficiency relative to u235 [kBq U235-Eq]": 0.2376969874398057,
        "EF v3.1 | land use | soil quality index [dimensionless]": 16.72946495654565,
        "EF v3.1 | material resources: metals/minerals | abiotic depletion potential (ADP): elements (ultimate reserves) [kg Sb-Eq]": 6.181291681542243e-05,
        "EF v3.1 | ozone depletion | ozone depletion potential (ODP) [kg CFC-11-Eq]": 2.406743135541314e-07,
        "EF v3.1 | particulate matter formation | impact on human health [disease incidence]": 2.437438102424734e-07,
        "EF v3.1 | photochemical oxidant formation: human health | tropospheric ozone concentration increase [kg NMVOC-Eq]": 0.02091633548598189,
        "EF v3.1 | water use | user deprivation potential (deprivation-weighted water consumption) [m3 world Eq deprived]": 1.587421316680642
      }
    },
    "ecoinvent_row_15528": {
      "matched_activity_name": "market for steel, low-alloyed, hot rolled",
      "matched_geography": "GLO",
      "match_confidence": "row_index (row 15528)",
      "selected_methodology": "ef31",
      "values": {
        "EF v3.1 | acidification | accumulated exceedance (AE) [mol H+-Eq]": 0.00923181934944304,
        "EF v3.1 | climate change | global warming potential (GWP100) [kg CO2-Eq]": 2.282166926427142,
        "EF v3.1 | climate change: biogenic | global warming potential (GWP100) [kg CO2-Eq]": 0.001755570624625085,
        "EF v3.1 | climate change: fossil | global warming potential (GWP100) [kg CO2-Eq]": 2.278895365610432,
        "EF v3.1 | climate change: land use and land use change | global warming potential (GWP100) [kg CO2-Eq]": 0.001515990192086111,
        "EF v3.1 | ecotoxicity: freshwater | comparative toxic unit for ecosystems (CTUe) [CTUe]": 15.62789394697456,
        "EF v3.1 | ecotoxicity: freshwater, inorganics | comparative toxic unit for ecosystems (CTUe) [CTUe]": 15.23331976838133,
        "EF v3.1 | ecotoxicity: freshwater, organics | comparative toxic unit for ecosystems (CTUe) [CTUe]": 0.3945741785932446,
        "EF v3.1 | energy resources: non-renewable | abiotic depletion potential (ADP): fossil fuels [MJ, net calorific value]": 24.79788622413608,
        "EF v3.1 | eutrophication: freshwater | fraction of nutrients reaching freshwater end compartment (P) [kg P-Eq]": 0.001285017120930655,
        "EF v3.1 | eutrophication: marine | fraction of nutrients reaching marine end compartment (N) [kg N-Eq]": 0.002206987926600248,
        "EF v3.1 | eutrophication: terrestrial | accumulated exceedance (AE) [mol N-Eq]": 0.02261596686421673,
        "EF v3.1 | human toxicity: carcinogenic | comparative toxic unit for human (CTUh) [CTUh]": 2.36731352025361e-09,
        "EF v3.1 | human toxicity: carcinogenic, inorganics | comparative toxic unit for human (CTUh) [CTUh]": 5.423190898452324e-10,
        "EF v3.1 | human toxicity: carcinogenic, organics | comparative toxic unit for human (CTUh) [CTUh]": 1.824994430408381e-09,
        "EF v3.1 | human toxicity: non-carcinogenic | comparative toxic unit for human (CTUh) [CTUh]": 4.099173235390985e-08,
        "EF v3.1 | human toxicity: non-carcinogenic, inorganics | comparative toxic unit for human (CTUh) [CTUh]": 3.990700579834342e-08,
        "EF v3.1 | human toxicity: non-carcinogenic, organics | comparative toxic unit for human (CTUh) [CTUh]": 1.084726555566458e-09,
        "EF v3.1 | ionising radiation: human health | human exposure efficiency relative to u235 [kBq U235-Eq]": 0.07925677499369514,
        "EF v3.1 | land use | soil quality index [dimensionless]": 7.743848201228083,
        "EF v3.1 | material resources: metals/minerals | abiotic depletion potential (ADP): elements (ultimate reserves) [kg Sb-Eq]": 1.597372828904201e-05,
        "EF v3.1 | ozone depletion | ozone depletion potential (ODP) [kg CFC-11-Eq]": 1.391687212152852e-08,
        "EF v3.1 | particulate matter formation | impact on human health [disease incidence]": 2.20267041140273e-07,
        "EF v3.1 | photochemical oxidant formation: human health | tropospheric ozone concentration increase [kg NMVOC-Eq]": 0.007905956222365838,
        "EF v3.1 | water use | user deprivation potential (deprivation-weighted water consumption) [m3 world Eq deprived]": 1.087320243222951
      }
    },
    "ecoinvent_row_9452": {
      "matched_activity_name": "market for aluminium, cast alloy",
      "matched_geography": "GLO",
      "match_confidence": "row_index (row 9452)",
      "selected_methodology": "ef31",
      "values": {
        "EF v3.1 | acidification | accumulated exceedance (AE) [mol H+-Eq]": 0.03932761918977569,
        "EF v3.1 | climate change | global warming potential (GWP100) [kg CO2-Eq]": 6.186142060241115,
        "EF v3.1 | climate change: biogenic | global warming potential (GWP100) [kg CO2-Eq]": 0.008760735554239986,
        "EF v3.1 | climate change: fossil | global warming potential (GWP100) [kg CO2-Eq]": 6.164567889673611,
        "EF v3.1 | climate change: land use and land use change | global warming potential (GWP100) [kg CO2-Eq]": 0.01281343501326624,
        "EF v3.1 | ecotoxicity: freshwater | comparative toxic unit for ecosystems (CTUe) [CTUe]": 33.86350766867174,
        "EF v3.1 | ecotoxicity: freshwater, inorganics | comparative toxic unit for ecosystems (CTUe) [CTUe]": 33.30965782822844,
        "EF v3.1 | ecotoxicity: freshwater, organics | comparative toxic unit for ecosystems (CTUe) [CTUe]": 0.553849840443304,
        "EF v3.1 | energy resources: non-renewable | abiotic depletion potential (ADP): fossil fuels [MJ, net calorific value]": 60.87921818613975,
        "EF v3.1 | eutrophication: freshwater | fraction of nutrients reaching freshwater end compartment (P) [kg P-Eq]": 0.002188109796025979,
        "EF v3.1 | eutrophication: marine | fraction of nutrients reaching marine end compartment (N) [kg N-Eq]": 0.00669937940736906,
        "EF v3.1 | eutrophication: terrestrial | accumulated exceedance (AE) [mol N-Eq]": 0.06941356829197398,
        "EF v3.1 | human toxicity: carcinogenic | comparative toxic unit for human (CTUh) [CTUh]": 4.237320782612722e-09,
        "EF v3.1 | human toxicity: carcinogenic, inorganics | comparative toxic unit for human (CTUh) [CTUh]": 1.245866119835258e-09,
        "EF v3.1 | human toxicity: carcinogenic, organics | comparative toxic unit for human (CTUh) [CTUh]": 2.991454662777463e-09,
        "EF v3.1 | human toxicity: non-carcinogenic | comparative toxic unit for human (CTUh) [CTUh]": 5.840537608378513e-08,
        "EF v3.1 | human toxicity: non-carcinogenic, inorganics | comparative toxic unit for human (CTUh) [CTUh]": 5.705120963378501e-08,
        "EF v3.1 | human toxicity: non-carcinogenic, organics | comparative toxic unit for human (CTUh) [CTUh]": 1.35416645000011e-09,
        "EF v3.1 | ionising radiation: human health | human exposure efficiency relative to u235 [kBq U235-Eq]": 0.1140012564763068,
        "EF v3.1 | land use | soil quality index [dimensionless]": 15.83280313372404,
        "EF v3.1 | material resources: metals/minerals | abiotic depletion potential (ADP): elements (ultimate reserves) [kg Sb-Eq]": 7.855621308369226e-05,
        "EF v3.1 | ozone depletion | ozone depletion potential (ODP) [kg CFC-11-Eq]": 3.823322054567926e-08,
        "EF v3.1 | particulate matter formation | impact on human health [disease incidence]": 5.186943090146374e-07,
        "EF v3.1 | photochemical oxidant formation: human health | tropospheric ozone concentration increase [kg NMVOC-Eq]": 0.02041588116879821,
        "EF v3.1 | water use | user deprivation potential (deprivation-weighted water consumption) [m3 world Eq deprived]": 1.641997086892984
      }
    },
    "ecoinvent_secondary_steel_electric_glo": {
      "matched_activity_name": "electric arc furnace secondary metallurgy slag to market for electric arc furnace secondary metallurgy slag for recovery",
      "matched_geography": "RoW",
      "match_confidence": "keyword (1 of 33 candidates)",
      "selected_methodology": "ef31",
      "values": {
        "EF v3.1 | acidification | accumulated exceedance (AE) [mol H+-Eq]": 0.0,
        "EF v3.1 | climate change | global warming potential (GWP100) [kg CO2-Eq]": 0.0,
        "EF v3.1 | climate change: biogenic | global warming potential (GWP100) [kg CO2-Eq]": 0.0,
        "EF v3.1 | climate change: fossil | global warming potential (GWP100) [kg CO2-Eq]": 0.0,
        "EF v3.1 | climate change: land use and land use change | global warming potential (GWP100) [kg CO2-Eq]": 0.0,
        "EF v3.1 | ecotoxicity: freshwater | comparative toxic unit for ecosystems (CTUe) [CTUe]": 0.0,
        "EF v3.1 | ecotoxicity: freshwater, inorganics | comparative toxic unit for ecosystems (CTUe) [CTUe]": 0.0,
        "EF v3.1 | ecotoxicity: freshwater, organics | comparative toxic unit for ecosystems (CTUe) [CTUe]": 0.0,
        "EF v3.1 | energy resources: non-renewable | abiotic depletion potential (ADP): fossil fuels [MJ, net calorific value]": 0.0,
        "EF v3.1 | eutrophication: freshwater | fraction of nutrients reaching freshwater end compartment (P) [kg P-Eq]": 0.0,
        "EF v3.1 | eutrophication: marine | fraction of nutrients reaching marine end compartment (N) [kg N-Eq]": 0.0,
        "EF v3.1 | eutrophication: terrestrial | accumulated exceedance (AE) [mol N-Eq]": 0.0,
        "EF v3.1 | human toxicity: carcinogenic | comparative toxic unit for human (CTUh) [CTUh]": 0.0,
        "EF v3.1 | human toxicity: carcinogenic, inorganics | comparative toxic unit for human (CTUh) [CTUh]": 0.0,
        "EF v3.1 | human toxicity: carcinogenic, organics | comparative toxic unit for human (CTUh) [CTUh]": 0.0,
        "EF v3.1 | human toxicity: non-carcinogenic | comparative toxic unit for human (CTUh) [CTUh]": 0.0,
        "EF v3.1 | human toxicity: non-carcinogenic, inorganics | comparative toxic unit for human (CTUh) [CTUh]": 0.0,
        "EF v3.1 | human toxicity: non-carcinogenic, organics | comparative toxic unit for human (CTUh) [CTUh]": 0.0,
        "EF v3.1 | ionising radiation: human health | human exposure efficiency relative to u235 [kBq U235-Eq]": 0.0,
        "EF v3.1 | land use | soil quality index [dimensionless]": 0.0,
        "EF v3.1 | material resources: metals/minerals | abiotic depletion potential (ADP): elements (ultimate reserves) [kg Sb-Eq]": 0.0,
        "EF v3.1 | ozone depletion | ozone depletion potential (ODP) [kg CFC-11-Eq]": 0.0,
        "EF v3.1 | particulate matter formation | impact on human health [disease incidence]": 0.0,
        "EF v3.1 | photochemical oxidant formation: human health | tropospheric ozone concentration increase [kg NMVOC-Eq]": 0.0,
        "EF v3.1 | water use | user deprivation potential (deprivation-weighted water consumption) [m3 world Eq deprived]": 0.0
      }
    },
    "ecoinvent_transport_container_ship_glo": {
      "matched_activity_name": "market for transport, freight, sea, container ship with reefer, heavy fuel oil, cooling",
      "matched_geography": "GLO",
      "match_confidence": "keyword (1 of 6 candidates)",
      "selected_methodology": "ef31",
      "values": {
        "EF v3.1 | acidification | accumulated exceedance (AE) [mol H+-Eq]": 0.0003150406934292181,
        "EF v3.1 | climate change | global warming potential (GWP100) [kg CO2-Eq]": 0.02205431115668184,
        "EF v3.1 | climate change: biogenic | global warming potential (GWP100) [kg CO2-Eq]": 1.813795266243502e-05,
        "EF v3.1 | climate change: fossil | global warming potential (GWP100) [kg CO2-Eq]": 0.02202664661624786,
        "EF v3.1 | climate change: land use and land use change | global warming potential (GWP100) [kg CO2-Eq]": 9.526587771543395e-06,
        "EF v3.1 | ecotoxicity: freshwater | comparative toxic unit for ecosystems (CTUe) [CTUe]": 0.04383947686846026,
        "EF v3.1 | ecotoxicity: freshwater, inorganics | comparative toxic unit for ecosystems (CTUe) [CTUe]": 0.04068196505028895,
        "EF v3.1 | ecotoxicity: freshwater, organics | comparative toxic unit for ecosystems (CTUe) [CTUe]": 0.003157511818171343,
        "EF v3.1 | energy resources: non-renewable | abiotic depletion potential (ADP): fossil fuels [MJ, net calorific value]": 0.2719610852812405,
        "EF v3.1 | eutrophication: freshwater | fraction of nutrients reaching freshwater end compartment (P) [kg P-Eq]": 1.360320448826937e-06,
        "EF v3.1 | eutrophication: marine | fraction of nutrients reaching marine end compartment (N) [kg N-Eq]": 0.0001345649259056561,
        "EF v3.1 | eutrophication: terrestrial | accumulated exceedance (AE) [mol N-Eq]": 0.001480379639754946,
        "EF v3.1 | human toxicity: carcinogenic | comparative toxic unit for human (CTUh) [CTUh]": 4.100322967993811e-12,
        "EF v3.1 | human toxicity: carcinogenic, inorganics | comparative toxic unit for human (CTUh) [CTUh]": 2.359763589420586e-12,
        "EF v3.1 | human toxicity: carcinogenic, organics | comparative toxic unit for human (CTUh) [CTUh]": 1.740559378573225e-12,
        "EF v3.1 | human toxicity: non-carcinogenic | comparative toxic unit for human (CTUh) [CTUh]": 8.93053321721101e-11,
        "EF v3.1 | human toxicity: non-carcinogenic, inorganics | comparative toxic unit for human (CTUh) [CTUh]": 8.354592209479726e-11,
        "EF v3.1 | human toxicity: non-carcinogenic, organics | comparative toxic unit for human (CTUh) [CTUh]": 5.759410077312811e-12,
        "EF v3.1 | ionising radiation: human health | human exposure efficiency relative to u235 [kBq U235-Eq]": 0.0001549163500951001,
        "EF v3.1 | land use | soil quality index [dimensionless]": 0.02383672483982366,
        "EF v3.1 | material resources: metals/minerals | abiotic depletion potential (ADP): elements (ultimate reserves) [kg Sb-Eq]": 8.678589809224939e-08,
        "EF v3.1 | ozone depletion | ozone depletion potential (ODP) [kg CFC-11-Eq]": 4.657448101525325e-10,
        "EF v3.1 | particulate matter formation | impact on human health [disease incidence]": 5.637697634897103e-10,
        "EF v3.1 | photochemical oxidant formation: human health | tropospheric ozone concentration increase [kg NMVOC-Eq]": 0.0004037318163076767,
        "EF v3.1 | water use | user deprivation potential (deprivation-weighted water consumption) [m3 world Eq deprived]": 0.001064348777179877
      }
    },
    "ecoinvent_transport_freight_train_rer": {
      "matched_activity_name": "market group for transport, freight, train, fleet average",
      "matched_geography": "RER",
      "match_confidence": "keyword",
      "selected_methodology": "ef31",
      "values": {
        "EF v3.1 | acidification | accumulated exceedance (AE) [mol H+-Eq]": 0.0003499459822998194,
        "EF v3.1 | climate change | global warming potential (GWP100) [kg CO2-Eq]": 0.04716369044991895,
        "EF v3.1 | climate change: biogenic | global warming potential (GWP100) [kg CO2-Eq]": 3.635149410981587e-05,
        "EF v3.1 | climate change: fossil | global warming potential (GWP100) [kg CO2-Eq]": 0.04706585476803656,
        "EF v3.1 | climate change: land use and land use change | global warming potential (GWP100) [kg CO2-Eq]": 6.148418777257255e-05,
        "EF v3.1 | ecotoxicity: freshwater | comparative toxic unit for ecosystems (CTUe) [CTUe]": 0.1731884580023237,
        "EF v3.1 | ecotoxicity: freshwater, inorganics | comparative toxic unit for ecosystems (CTUe) [CTUe]": 0.1685692897778814,
        "EF v3.1 | ecotoxicity: freshwater, organics | comparative toxic unit for ecosystems (CTUe) [CTUe]": 0.004619168224442386,
        "EF v3.1 | energy resources: non-renewable | abiotic depletion potential (ADP): fossil fuels [MJ, net calorific value]": 0.6741395379144332,
        "EF v3.1 | eutrophication: freshwater | fraction of nutrients reaching freshwater end compartment (P) [kg P-Eq]": 1.651759676756538e-05,
        "EF v3.1 | eutrophication: marine | fraction of nutrients reaching marine end compartment (N) [kg N-Eq]": 0.0001334344671556992,
        "EF v3.1 | eutrophication: terrestrial | accumulated exceedance (AE) [mol N-Eq]": 0.001432748075274211,
        "EF v3.1 | human toxicity: carcinogenic | comparative toxic unit for human (CTUh) [CTUh]": 1.183355801814533e-11,
        "EF v3.1 | human toxicity: carcinogenic, inorganics | comparative toxic unit for human (CTUh) [CTUh]": 4.353602855505371e-12,
        "EF v3.1 | human toxicity: carcinogenic, organics | comparative toxic unit for human (CTUh) [CTUh]": 7.479955162639956e-12,
        "EF v3.1 | human toxicity: non-carcinogenic | comparative toxic unit for human (CTUh) [CTUh]": 3.574028053583227e-10,
        "EF v3.1 | human toxicity: non-carcinogenic, inorganics | comparative toxic unit for human (CTUh) [CTUh]": 3.381471592997696e-10,
        "EF v3.1 | human toxicity: non-carcinogenic, organics | comparative toxic unit for human (CTUh) [CTUh]": 1.925564605855342e-11,
        "EF v3.1 | ionising radiation: human health | human exposure efficiency relative to u235 [kBq U235-Eq]": 0.006831958246451759,
        "EF v3.1 | land use | soil quality index [dimensionless]": 0.4380841298971929,
        "EF v3.1 | material resources: metals/minerals | abiotic depletion potential (ADP): elements (ultimate reserves) [kg Sb-Eq]": 1.453242335056268e-07,
        "EF v3.1 | ozone depletion | ozone depletion potential (ODP) [kg CFC-11-Eq]": 7.454959677963208e-10,
        "EF v3.1 | particulate matter formation | impact on human health [disease incidence]": 4.536063288247527e-09,
        "EF v3.1 | photochemical oxidant formation: human health | tropospheric ozone concentration increase [kg NMVOC-Eq]": 0.0004218253275585902,
        "EF v3.1 | water use | user deprivation potential (deprivation-weighted water consumption) [m3 world Eq deprived]": 0.01266683543187878
      }
    },
    "ecoinvent_transport_lorry_32t_rer": {
      "matched_activity_name": "market for transport, freight, lorry, 16-32 metric ton, diesel, EURO 3",
      "matched_geography": "RER",
      "match_confidence": "keyword (1 of 37 candidates)",
      "selected_methodology": "ef31",
      "values": {
        "EF v3.1 | acidification | accumulated exceedance (AE) [mol H+-Eq]": 0.001053563456189026,
        "EF v3.1 | climate change | global warming potential (GWP100) [kg CO2-Eq]": 0.1906690452621614,
        "EF v3.1 | climate change: biogenic | global warming potential (GWP100) [kg CO2-Eq]": 3.598832950844442e-05,
        "EF v3.1 | climate change: fossil | global warming potential (GWP100) [kg CO2-Eq]": 0.1905716069843386,
        "EF v3.1 | climate change: land use and land use change | global warming potential (GWP100) [kg CO2-Eq]": 6.144994831441361e-05,
        "EF v3.1 | ecotoxicity: freshwater | comparative toxic unit for ecosystems (CTUe) [CTUe]": 0.4006037162231726,
        "EF v3.1 | ecotoxicity: freshwater, inorganics | comparative toxic unit for ecosystems (CTUe) [CTUe]": 0.3809467586050359,
        "EF v3.1 | ecotoxicity: freshwater, organics | comparative toxic unit for ecosystems (CTUe) [CTUe]": 0.019656957618137,
        "EF v3.1 | energy resources: non-renewable | abiotic depletion potential (ADP): fossil fuels [MJ, net calorific value]": 2.706799996532563,
        "EF v3.1 | eutrophication: freshwater | fraction of nutrients reaching freshwater end compartment (P) [kg P-Eq]": 1.323598825663963e-05,
        "EF v3.1 | eutrophication: marine | fraction of nutrients reaching marine end compartment (N) [kg N-Eq]": 0.0004477093015982698,
        "EF v3.1 | eutrophication: terrestrial | accumulated exceedance (AE) [mol N-Eq]": 0.00488221516499021,
        "EF v3.1 | human toxicity: carcinogenic | comparative toxic unit for human (CTUh) [CTUh]": 7.144599163356931e-11,
        "EF v3.1 | human toxicity: carcinogenic, inorganics | comparative toxic unit for human (CTUh) [CTUh]": 1.265793942719845e-11,
        "EF v3.1 | human toxicity: carcinogenic, organics | comparative toxic unit for human (CTUh) [CTUh]": 5.878805220637083e-11,
        "EF v3.1 | human toxicity: non-carcinogenic | comparative toxic unit for human (CTUh) [CTUh]": 2.102300987793302e-09,
        "EF v3.1 | human toxicity: non-carcinogenic, inorganics | comparative toxic unit for human (CTUh) [CTUh]": 1.519657372216476e-09,
        "EF v3.1 | human toxicity: non-carcinogenic, organics | comparative toxic unit for human (CTUh) [CTUh]": 5.826436155768269e-10,
        "EF v3.1 | ionising radiation: human health | human exposure efficiency relative to u235 [kBq U235-Eq]": 0.003075035708473385,
        "EF v3.1 | land use | soil quality index [dimensionless]": 1.597641520863033,
        "EF v3.1 | material resources: metals/minerals | abiotic depletion potential (ADP): elements (ultimate reserves) [kg Sb-Eq]": 6.631716830975347e-07,
        "EF v3.1 | ozone depletion | ozone depletion potential (ODP) [kg CFC-11-Eq]": 4.34026203283501e-09,
        "EF v3.1 | particulate matter formation | impact on human health [disease incidence]": 2.058762921709348e-08,
        "EF v3.1 | photochemical oxidant formation: human health | tropospheric ozone concentration increase [kg NMVOC-Eq]": 0.001598207520660874,
        "EF v3.1 | water use | user deprivation potential (deprivation-weighted water consumption) [m3 world Eq deprived]": 0.01400042286198134
      }
    },
    "ecoinvent_virgin_steel_primary_glo": {
      "matched_activity_name": "abrasive blasting, alumina, carbon steel substrate",
      "matched_geography": "GLO",
      "match_confidence": "keyword (1 of 731 candidates)",
      "selected_methodology": "ef31",
      "values": {
        "EF v3.1 | acidification | accumulated exceedance (AE) [mol H+-Eq]": 0.1168800340387907,
        "EF v3.1 | climate change | global warming potential (GWP100) [kg CO2-Eq]": 21.78981028667413,
        "EF v3.1 | climate change: biogenic | global warming potential (GWP100) [kg CO2-Eq]": 0.03376897904385948,
        "EF v3.1 | climate change: fossil | global warming potential (GWP100) [kg CO2-Eq]": 21.7129053996283,
        "EF v3.1 | climate change: land use and land use change | global warming potential (GWP100) [kg CO2-Eq]": 0.04313590800197154,
        "EF v3.1 | ecotoxicity: freshwater | comparative toxic unit for ecosystems (CTUe) [CTUe]": 65.77462008694926,
        "EF v3.1 | ecotoxicity: freshwater, inorganics | comparative toxic unit for ecosystems (CTUe) [CTUe]": 63.53556433613577,
        "EF v3.1 | ecotoxicity: freshwater, organics | comparative toxic unit for ecosystems (CTUe) [CTUe]": 2.239055750813729,
        "EF v3.1 | energy resources: non-renewable | abiotic depletion potential (ADP): fossil fuels [MJ, net calorific value]": 293.1864462234327,
        "EF v3.1 | eutrophication: freshwater | fraction of nutrients reaching freshwater end compartment (P) [kg P-Eq]": 0.0110171438294262,
        "EF v3.1 | eutrophication: marine | fraction of nutrients reaching marine end compartment (N) [kg N-Eq]": 0.02277191930444603,
        "EF v3.1 | eutrophication: terrestrial | accumulated exceedance (AE) [mol N-Eq]": 0.2290528510308444,
        "EF v3.1 | human toxicity: carcinogenic | comparative toxic unit for human (CTUh) [CTUh]": 4.333819387940363e-09,
        "EF v3.1 | human toxicity: carcinogenic, inorganics | comparative toxic unit for human (CTUh) [CTUh]": 2.658235247544462e-09,
        "EF v3.1 | human toxicity: carcinogenic, organics | comparative toxic unit for human (CTUh) [CTUh]": 1.675584140395902e-09,
        "EF v3.1 | human toxicity: non-carcinogenic | comparative toxic unit for human (CTUh) [CTUh]": 2.119779249949037e-07,
        "EF v3.1 | human toxicity: non-carcinogenic, inorganics | comparative toxic unit for human (CTUh) [CTUh]": 2.042757072434386e-07,
        "EF v3.1 | human toxicity: non-carcinogenic, organics | comparative toxic unit for human (CTUh) [CTUh]": 7.702217751465351e-09,
        "EF v3.1 | ionising radiation: human health | human exposure efficiency relative to u235 [kBq U235-Eq]": 3.15011042946511,
        "EF v3.1 | land use | soil quality index [dimensionless]": 53.49758053202067,
        "EF v3.1 | material resources: metals/minerals | abiotic depletion potential (ADP): elements (ultimate reserves) [kg Sb-Eq]": 0.0001173066486080051,
        "EF v3.1 | ozone depletion | ozone depletion potential (ODP) [kg CFC-11-Eq]": 1.676067265362502e-07,
        "EF v3.1 | particulate matter formation | impact on human health [disease incidence]": 1.101060748143439e-06,
        "EF v3.1 | photochemical oxidant formation: human health | tropospheric ozone concentration increase [kg NMVOC-Eq]": 0.06665989054515836,
        "EF v3.1 | water use | user deprivation potential (deprivation-weighted water consumption) [m3 world Eq deprived]": 5.755961978057131
      }
    },
    "ecoinvent_waste_incineration_glo": {
      "matched_activity_name": "electricity, from municipal waste incineration to generic market for electricity, medium voltage",
      "matched_geography": "AT",
      "match_confidence": "keyword (1 of 740 candidates)",
      "selected_methodology": "ef31",
      "values": {
        "EF v3.1 | acidification | accumulated exceedance (AE) [mol H+-Eq]": 0.0,
        "EF v3.1 | climate change | global warming potential (GWP100) [kg CO2-Eq]": 0.0,
        "EF v3.1 | climate change: biogenic | global warming potential (GWP100) [kg CO2-Eq]": 0.0,
        "EF v3.1 | climate change: fossil | global warming potential (GWP100) [kg CO2-Eq]": 0.0,
        "EF v3.1 | climate change: land use and land use change | global warming potential (GWP100) [kg CO2-Eq]": 0.0,
        "EF v3.1 | ecotoxicity: freshwater | comparative toxic unit for ecosystems (CTUe) [CTUe]": 0.0,
        "EF v3.1 | ecotoxicity: freshwater, inorganics | comparative toxic unit for ecosystems (CTUe) [CTUe]": 0.0,
        "EF v3.1 | ecotoxicity: freshwater, organics | comparative toxic unit for ecosystems (CTUe) [CTUe]": 0.0,
        "EF v3.1 | energy resources: non-renewable | abiotic depletion potential (ADP): fossil fuels [MJ, net calorific value]": 0.0,
        "EF v3.1 | eutrophication: freshwater | fraction of nutrients reaching freshwater end compartment (P) [kg P-Eq]": 0.0,
        "EF v3.1 | eutrophication: marine | fraction of nutrients reaching marine end compartment (N) [kg N-Eq]": 0.0,
        "EF v3.1 | eutrophication: terrestrial | accumulated exceedance (AE) [mol N-Eq]": 0.0,
        "EF v3.1 | human toxicity: carcinogenic | comparative toxic unit for human (CTUh) [CTUh]": 0.0,
        "EF v3.1 | human toxicity: carcinogenic, inorganics | comparative toxic unit for human (CTUh) [CTUh]": 0.0,
        "EF v3.1 | human toxicity: carcinogenic, organics | comparative toxic unit for human (CTUh) [CTUh]": 0.0,
        "EF v3.1 | human toxicity: non-carcinogenic | comparative toxic unit for human (CTUh) [CTUh]": 0.0,
        "EF v3.1 | human toxicity: non-carcinogenic, inorganics | comparative toxic unit for human (CTUh) [CTUh]": 0.0,
        "EF v3.1 | human toxicity: non-carcinogenic, organics | comparative toxic unit for human (CTUh) [CTUh]": 0.0,
        "EF v3.1 | ionising radiation: human health | human exposure efficiency relative to u235 [kBq U235-Eq]": 0.0,
        "EF v3.1 | land use | soil quality index [dimensionless]": 0.0,
        "EF v3.1 | material resources: metals/minerals | abiotic depletion potential (ADP): elements (ultimate reserves) [kg Sb-Eq]": 0.0,
        "EF v3.1 | ozone depletion | ozone depletion potential (ODP) [kg CFC-11-Eq]": 0.0,
        "EF v3.1 | particulate matter formation | impact on human health [disease incidence]": 0.0,
        "EF v3.1 | photochemical oxidant formation: human health | tropospheric ozone concentration increase [kg NMVOC-Eq]": 0.0,
        "EF v3.1 | water use | user deprivation potential (deprivation-weighted water consumption) [m3 world Eq deprived]": 0.0
      }
    },
    "ecoinvent_waste_landfill_glo": {
      "matched_activity_name": "treatment of basic oxygen furnace waste, residual material landfill",
      "matched_geography": "RoW",
      "match_confidence": "keyword (1 of 537 candidates)",
      "selected_methodology": "ef31",
      "values": {
        "EF v3.1 | acidification | accumulated exceedance (AE) [mol H+-Eq]": 0.001092284735263689,
        "EF v3.1 | climate change | global warming potential (GWP100) [kg CO2-Eq]": 0.3435347873560755,
        "EF v3.1 | climate change: biogenic | global warming potential (GWP100) [kg CO2-Eq]": 0.00035980853321476,
        "EF v3.1 | climate change: fossil | global warming potential (GWP100) [kg CO2-Eq]": 0.3430717557833489,
        "EF v3.1 | climate change: land use and land use change | global warming potential (GWP100) [kg CO2-Eq]": 0.0001032230395119429,
        "EF v3.1 | ecotoxicity: freshwater | comparative toxic unit for ecosystems (CTUe) [CTUe]": 1.037320275729926,
        "EF v3.1 | ecotoxicity: freshwater, inorganics | comparative toxic unit for ecosystems (CTUe) [CTUe]": 1.020671061672707,
        "EF v3.1 | ecotoxicity: freshwater, organics | comparative toxic unit for ecosystems (CTUe) [CTUe]": 0.01664921405722022,
        "EF v3.1 | energy resources: non-renewable | abiotic depletion potential (ADP): fossil fuels [MJ, net calorific value]": 1.91123668657653,
        "EF v3.1 | eutrophication: freshwater | fraction of nutrients reaching freshwater end compartment (P) [kg P-Eq]": 0.006580262834395015,
        "EF v3.1 | eutrophication: marine | fraction of nutrients reaching marine end compartment (N) [kg N-Eq]": 0.0003358214561775645,
        "EF v3.1 | eutrophication: terrestrial | accumulated exceedance (AE) [mol N-Eq]": 0.00374215435815483,
        "EF v3.1 | human toxicity: carcinogenic | comparative toxic unit for human (CTUh) [CTUh]": 2.197731198504857e-09,
        "EF v3.1 | human toxicity: carcinogenic, inorganics | comparative toxic unit for human (CTUh) [CTUh]": 2.166328272566605e-09,
        "EF v3.1 | human toxicity: carcinogenic, organics | comparative toxic unit for human (CTUh) [CTUh]": 3.140292593825091e-11,
        "EF v3.1 | human toxicity: non-carcinogenic | comparative toxic unit for human (CTUh) [CTUh]": 2.345035685298958e-09,
        "EF v3.1 | human toxicity: non-carcinogenic, inorganics | comparative toxic unit for human (CTUh) [CTUh]": 2.289153316977927e-09,
        "EF v3.1 | human toxicity: non-carcinogenic, organics | comparative toxic unit for human (CTUh) [CTUh]": 5.588236832103174e-11,
        "EF v3.1 | ionising radiation: human health | human exposure efficiency relative to u235 [kBq U235-Eq]": 0.003116786330020858,
        "EF v3.1 | land use | soil quality index [dimensionless]": 1.780040073696534,
        "EF v3.1 | material resources: metals/minerals | abiotic depletion potential (ADP): elements (ultimate reserves) [kg Sb-Eq]": 1.56375206143482e-06,
        "EF v3.1 | ozone depletion | ozone depletion potential (ODP) [kg CFC-11-Eq]": 1.488459534598485e-09,
        "EF v3.1 | particulate matter formation | impact on human health [disease incidence]": 1.19237222412867e-08,
        "EF v3.1 | photochemical oxidant formation: human health | tropospheric ozone concentration increase [kg NMVOC-Eq]": 0.00106180076782536,
        "EF v3.1 | water use | user deprivation potential (deprivation-weighted water consumption) [m3 world Eq deprived]": 0.0373364151554146
      }
    },
    "ecoinvent_waste_metal_recycling_glo": {
      "matched_activity_name": "container production, for collection of post-consumer waste plastic for recycling",
      "matched_geography": "CH",
      "match_confidence": "keyword (1 of 225 candidates)",
      "selected_methodology": "ef31",
      "values": {
        "EF v3.1 | acidification | accumulated exceedance (AE) [mol H+-Eq]": 0.0002045130350381118,
        "EF v3.1 | climate change | global warming potential (GWP100) [kg CO2-Eq]": 0.05948079957374758,
        "EF v3.1 | climate change: biogenic | global warming potential (GWP100) [kg CO2-Eq]": 5.860927856112916e-05,
        "EF v3.1 | climate change: fossil | global warming potential (GWP100) [kg CO2-Eq]": 0.05935275487498795,
        "EF v3.1 | climate change: land use and land use change | global warming potential (GWP100) [kg CO2-Eq]": 6.943542019849475e-05,
        "EF v3.1 | ecotoxicity: freshwater | comparative toxic unit for ecosystems (CTUe) [CTUe]": 0.2823075270634108,
        "EF v3.1 | ecotoxicity: freshwater, inorganics | comparative toxic unit for ecosystems (CTUe) [CTUe]": 0.2647417394873714,
        "EF v3.1 | ecotoxicity: freshwater, organics | comparative toxic unit for ecosystems (CTUe) [CTUe]": 0.01756578757603918,
        "EF v3.1 | energy resources: non-renewable | abiotic depletion potential (ADP): fossil fuels [MJ, net calorific value]": 1.587690362418939,
        "EF v3.1 | eutrophication: freshwater | fraction of nutrients reaching freshwater end compartment (P) [kg P-Eq]": 2.164213038156823e-05,
        "EF v3.1 | eutrophication: marine | fraction of nutrients reaching marine end compartment (N) [kg N-Eq]": 4.731303039827288e-05,
        "EF v3.1 | eutrophication: terrestrial | accumulated exceedance (AE) [mol N-Eq]": 0.000460993405041774,
        "EF v3.1 | human toxicity: carcinogenic | comparative toxic unit for human (CTUh) [CTUh]": 2.13645091653686e-11,
        "EF v3.1 | human toxicity: carcinogenic, inorganics | comparative toxic unit for human (CTUh) [CTUh]": 8.07100741875612e-12,
        "EF v3.1 | human toxicity: carcinogenic, organics | comparative toxic unit for human (CTUh) [CTUh]": 1.329350174661249e-11,
        "EF v3.1 | human toxicity: non-carcinogenic | comparative toxic unit for human (CTUh) [CTUh]": 5.244696400199347e-10,
        "EF v3.1 | human toxicity: non-carcinogenic, inorganics | comparative toxic unit for human (CTUh) [CTUh]": 4.893504183656601e-10,
        "EF v3.1 | human toxicity: non-carcinogenic, organics | comparative toxic unit for human (CTUh) [CTUh]": 3.511922165427446e-11,
        "EF v3.1 | ionising radiation: human health | human exposure efficiency relative to u235 [kBq U235-Eq]": 0.008218491383525085,
        "EF v3.1 | land use | soil quality index [dimensionless]": 0.272507382261674,
        "EF v3.1 | material resources: metals/minerals | abiotic depletion potential (ADP): elements (ultimate reserves) [kg Sb-Eq]": 4.653913742800084e-07,
        "EF v3.1 | ozone depletion | ozone depletion potential (ODP) [kg CFC-11-Eq]": 2.83962119578066e-09,
        "EF v3.1 | particulate matter formation | impact on human health [disease incidence]": 1.931852134051705e-09,
        "EF v3.1 | photochemical oxidant formation: human health | tropospheric ozone concentration increase [kg NMVOC-Eq]": 0.0003178857155204092,
        "EF v3.1 | water use | user deprivation potential (deprivation-weighted water consumption) [m3 world Eq deprived]": 0.03865293173589551
      }
    },
    "ecoinvent_water_deionised_glo": {
      "matched_activity_name": "market for water, deionised",
      "matched_geography": "CH",
      "match_confidence": "keyword (1 of 6 candidates)",
      "selected_methodology": "ef31",
      "values": {
        "EF v3.1 | acidification | accumulated exceedance (AE) [mol H+-Eq]": 3.893228489607181e-06,
        "EF v3.1 | climate change | global warming potential (GWP100) [kg CO2-Eq]": 0.0003109998299436259,
        "EF v3.1 | climate change: biogenic | global warming potential (GWP100) [kg CO2-Eq]": 3.42769506166786e-05,
        "EF v3.1 | climate change: fossil | global warming potential (GWP100) [kg CO2-Eq]": 0.0002764329259053298,
        "EF v3.1 | climate change: land use and land use change | global warming potential (GWP100) [kg CO2-Eq]": 2.899534216175466e-07,
        "EF v3.1 | ecotoxicity: freshwater | comparative toxic unit for ecosystems (CTUe) [CTUe]": 0.05062253824425585,
        "EF v3.1 | ecotoxicity: freshwater, inorganics | comparative toxic unit for ecosystems (CTUe) [CTUe]": 0.05054643707641698,
        "EF v3.1 | ecotoxicity: freshwater, organics | comparative toxic unit for ecosystems (CTUe) [CTUe]": 7.61011678390143e-05,
        "EF v3.1 | energy resources: non-renewable | abiotic depletion potential (ADP): fossil fuels [MJ, net calorific value]": 0.004045203228932253,
        "EF v3.1 | eutrophication: freshwater | fraction of nutrients reaching freshwater end compartment (P) [kg P-Eq]": 1.46133895928643e-07,
        "EF v3.1 | eutrophication: marine | fraction of nutrients reaching marine end compartment (N) [kg N-Eq]": 2.796085722752741e-07,
        "EF v3.1 | eutrophication: terrestrial | accumulated exceedance (AE) [mol N-Eq]": 2.721067590976641e-06,
        "EF v3.1 | human toxicity: carcinogenic | comparative toxic unit for human (CTUh) [CTUh]": 8.838111985565098e-13,
        "EF v3.1 | human toxicity: carcinogenic, inorganics | comparative toxic unit for human (CTUh) [CTUh]": 8.917464878614131e-14,
        "EF v3.1 | human toxicity: carcinogenic, organics | comparative toxic unit for human (CTUh) [CTUh]": 7.946365497703688e-13,
        "EF v3.1 | human toxicity: non-carcinogenic | comparative toxic unit for human (CTUh) [CTUh]": 5.507406251510176e-12,
        "EF v3.1 | human toxicity: non-carcinogenic, inorganics | comparative toxic unit for human (CTUh) [CTUh]": 5.181291298910631e-12,
        "EF v3.1 | human toxicity: non-carcinogenic, organics | comparative toxic unit for human (CTUh) [CTUh]": 3.261149525995438e-13,
        "EF v3.1 | ionising radiation: human health | human exposure efficiency relative to u235 [kBq U235-Eq]": 5.397890126312467e-05,
        "EF v3.1 | land use | soil quality index [dimensionless]": 0.001653967557560829,
        "EF v3.1 | material resources: metals/minerals | abiotic depletion potential (ADP): elements (ultimate reserves) [kg Sb-Eq]": 8.945724267980501e-09,
        "EF v3.1 | ozone depletion | ozone depletion potential (ODP) [kg CFC-11-Eq]": 1.52071544290178e-10,
        "EF v3.1 | particulate matter formation | impact on human health [disease incidence]": 3.100481660884286e-11,
        "EF v3.1 | photochemical oxidant formation: human health | tropospheric ozone concentration increase [kg NMVOC-Eq]": 1.051450511191681e-06,
        "EF v3.1 | water use | user deprivation potential (deprivation-weighted water consumption) [m3 world Eq deprived]": 0.000918464087906531
      }
    }
  }
}